@prefix rdf: <http://www.w3.org/1999/02/22-rdf-syntax-ns#> .
@prefix rdfs: <http://www.w3.org/2000/01/rdf-schema#> .
@prefix owl: <http://www.w3.org/2002/07/owl#> .
@prefix xsd: <http://www.w3.org/2001/XMLSchema#> .
@prefix xml: <http://www.w3.org/XML/1998/namespace/> .
@prefix mms-ontology: <https://opencae.jpl.nasa.gov/mms/rdf/ontology/> .
@prefix mms-graph: <https://opencae.jpl.nasa.gov/mms/rdf/graph/> .
@prefix mms-property: <https://opencae.jpl.nasa.gov/mms/rdf/property/> .
@prefix mms-derived-property: <https://opencae.jpl.nasa.gov/mms/rdf/derived-property/> .
@prefix mms-class: <https://opencae.jpl.nasa.gov/mms/rdf/class/> .
@prefix mms-element: <https://opencae.jpl.nasa.gov/mms/rdf/element/> .
@prefix mms-artifact: <https://opencae.jpl.nasa.gov/mms/rdf/artifact/> .
@prefix mms-index: <https://opencae.jpl.nasa.gov/mms/rdf/index/> .
@prefix mms-shape: <https://opencae.jpl.nasa.gov/mms/rdf/shape/> .
@prefix xmi: <http://www.omg.org/spec/XMI/20131001#> .
@prefix uml: <http://www.omg.org/spec/UML/20161101#> .
@prefix uml-model: <https://www.omg.org/spec/UML/20161101/UML.xmi#> .
@prefix uml-model-dt: <https://www.omg.org/spec/UML/20161101/UML.xmi#datatype/> .
@prefix uml-primitives: <https://www.omg.org/spec/UML/20161101/PrimitiveTypes.xmi#> .
@prefix uml-class: <https://opencae.jpl.nasa.gov/mms/rdf/uml-class/> .
@prefix uml-property: <https://opencae.jpl.nasa.gov/mms/rdf/uml-property/> .

mms-class:Element a owl:Class ;
	rdfs:label "Element" ;
	owl:equivalentClass uml-class:Element ;
	mms-ontology:category mms-class:Element .

mms-class:Commit a owl:Class ;
	rdfs:label "Commit" ;
	mms-ontology:category mms-class:Artifact .

mms-class:Ref a owl:Class ;
	rdfs:label "Ref" ;
	mms-ontology:category mms-class:Artifact .

mms-class:Project a owl:Class ;
	rdfs:label "Project" ;
	mms-ontology:category mms-class:Artifact .

mms-ontology:Property a owl:Class ;
	rdfs:label "Property" .

mms-class:PropertyPath a owl:Class ;
	rdfs:label "Property Path" ;
	mms-ontology:category mms-class:ElementList .

mms-ontology:ObjectProperty a owl:Class ;
	rdfs:label "Object Property" ;
	owl:equivalentClass owl:ObjectProperty ;
	rdfs:subClassOf mms-ontology:Property .

mms-ontology:DatatypeProperty a owl:Class ;
	rdfs:label "Datatype Property" ;
	owl:equivalentClass owl:DatatypeProperty ;
	rdfs:subClassOf mms-ontology:Property .

mms-ontology:UmlObjectProperty a owl:Class ;
	rdfs:label "UML Object Property" ;
	rdfs:subClassOf mms-ontology:ObjectProperty .

mms-ontology:UmlDatatypeProperty a owl:Class ;
	rdfs:label "UML Datatype Property" ;
	rdfs:subClassOf mms-ontology:DatatypeProperty .

mms-ontology:DerivedObjectProperty a owl:Class ;
	rdfs:label "Derived Object Property" ;
	rdfs:subClassOf mms-ontology:ObjectProperty .

mms-ontology:DerivedDatatypeProperty a owl:Class ;
	rdfs:label "Derived Datatype Property" ;
	rdfs:subClassOf mms-ontology:DatatypeProperty .

# a datatype restriction for properties with langString ranges
mms-ontology:Comment_EN owl:equivalentClass [
		rdf:type rdfs:Datatype ;
		owl:onDatatype rdfs:langString ;
		owl:withRestrictions (
			[
				xml:lang "en"^^xsd:language ;
			]
		) ;
	] .

# an enumerated class declaration for types of visibility
mms-class:Visibility a mms-ontology:EnumeratedClass ;
	mms-ontology:category mms-class:Element ;
	owl:oneOf (
		mms-class:Visibility.Public
		mms-class:Visibility.Private
		mms-class:Visibility.None
	) .

mms-class:Visibility.Public a owl:Class ;
	mms-ontology:enumerationValue "public" ;
	mms-ontology:category mms-class:Element .

mms-class:Visibility.Private a owl:Class ;
	mms-ontology:enumerationValue "private" ;
	mms-ontology:category mms-class:Element .

mms-class:Visibility.None a owl:Class ;
	mms-ontology:enumerationValue rdf:nil ;
	mms-ontology:category mms-class:Element .

mms-derived-property:appliedStereotypes a mms-ontology:DerivedObjectProperty ;
	mms-ontology:key "_appliedStereotypeIds" ;
	rdfs:label "appliedStereotype" ;
	rdfs:comment "List of AppliedStereotypes that belong to this Element. Based on the derived property '_appliedStereotypeIds'."@en ;
	rdfs:domain mms-class:Element ;
	rdfs:range mms-class:AppliedStereotypesList ;
	mms-ontology:listItemRange mms-class:AppliedStereotype ;
	mms-ontology:mappingDomain mms-class:Element .

mms-class:AppliedStereotypesList a owl:Class ;
	mms-ontology:category mms-class:ElementList ;
	rdfs:subClassOf [
		rdf:type owl:Class ;
		owl:intersectionOf (
			rdf:List
			[
				rdf:type owl:Restriction ;
				owl:onProperty rdf:first ;
				owl:allValuesFrom mms-class:AppliedStereotype ;
			]
			[
				rdf:type owl:Restriction ;
				owl:onProperty rdf:rest ;
				owl:allValuesFrom mms-class:AppliedStereotypesList ;
			]
		) ;
	] .

mms-derived-property:commit a mms-ontology:DerivedObjectProperty ;
	mms-ontology:key "_commitId" ;
	rdfs:label "commit" ;
	rdfs:comment "Based on the derived property '_commitId'."@en ;
	rdfs:domain mms-class:Element ;
	rdfs:range mms-class:Commit ;
	mms-ontology:mappingDomain mms-class:Element .

mms-derived-property:created a mms-ontology:DerivedDatatypeProperty ;
	mms-ontology:key "_created" ;
	rdfs:label "created" ;
	rdfs:comment "Based on the key '_created'"@en ;
	rdfs:domain mms-class:Element ;
	rdfs:range xsd:dateTime ;
	mms-ontology:mappingDomain mms-class:Element .

mms-derived-property:creator a mms-ontology:DerivedObjectProperty ;
	mms-ontology:key "_creator" ;
	rdfs:label "creator" ;
	rdfs:comment "The user who created this Element"@en ;
	rdfs:domain mms-class:Element ;
	mms-ontology:mappingDomain mms-class:Element ;
	rdfs:range mms-ontology:User .

mms-derived-property:diagramType a mms-ontology:DerivedDatatypeProperty ;
	mms-ontology:key "_diagramType" ;
	rdfs:label "diagramType" ;
	rdfs:comment "Based on the key '_diagramType'"@en ;
	rdfs:domain mms-class:Element ;
	rdfs:range xsd:string ;
	mms-ontology:mappingDomain mms-class:Element .

mms-derived-property:displayedElements a mms-ontology:DerivedObjectProperty ;
	mms-ontology:key "_displayedElementIds" ;
	rdfs:label "displayedElement" ;
	rdfs:comment "List of DisplayedElements that belong to this Element. Based on the derived property '_displayedElementIds'."@en ;
	rdfs:domain mms-class:Element ;
	rdfs:range mms-class:DisplayedElementsList ;
	mms-ontology:listItemRange mms-class:DisplayedElement ;
	mms-ontology:mappingDomain mms-class:Element .

mms-class:DisplayedElementsList a owl:Class ;
	mms-ontology:category mms-class:ElementList ;
	rdfs:subClassOf [
		rdf:type owl:Class ;
		owl:intersectionOf (
			rdf:List
			[
				rdf:type owl:Restriction ;
				owl:onProperty rdf:first ;
				owl:allValuesFrom mms-class:DisplayedElement ;
			]
			[
				rdf:type owl:Restriction ;
				owl:onProperty rdf:rest ;
				owl:allValuesFrom mms-class:DisplayedElementsList ;
			]
		) ;
	] .

mms-derived-property:editable a mms-ontology:DerivedDatatypeProperty ;
	mms-ontology:key "_editable" ;
	rdfs:label "editable" ;
	rdfs:comment "Based on the key '_editable'"@en ;
	rdfs:domain mms-class:Element ;
	rdfs:range xsd:boolean ;
	mms-ontology:mappingDomain mms-class:Element .

mms-derived-property:elastic a mms-ontology:DerivedObjectProperty ;
	mms-ontology:key "_elasticId" ;
	rdfs:label "elastic" ;
	rdfs:comment "Based on the derived property '_elasticId'."@en ;
	rdfs:domain mms-class:Element ;
	rdfs:range mms-class:Elastic ;
	mms-ontology:mappingDomain mms-class:Element .

mms-derived-property:group a mms-ontology:DerivedObjectProperty ;
	mms-ontology:key "_groupId" ;
	rdfs:label "group" ;
	rdfs:comment "Based on the derived property '_groupId'."@en ;
	rdfs:domain mms-class:Element ;
	rdfs:range mms-class:Group ;
	mms-ontology:mappingDomain mms-class:Element .

mms-derived-property:inRefs a mms-ontology:DerivedObjectProperty ;
	mms-ontology:key "_inRefIds" ;
	rdfs:label "inRef" ;
	rdfs:comment "List of InRefs that belong to this Element. Based on the derived property '_inRefIds'."@en ;
	rdfs:domain mms-class:Element ;
	rdfs:range mms-class:InRefsList ;
	mms-ontology:listItemRange mms-class:InRef ;
	mms-ontology:mappingDomain mms-class:Element .

mms-class:InRefsList a owl:Class ;
	mms-ontology:category mms-class:ElementList ;
	rdfs:subClassOf [
		rdf:type owl:Class ;
		owl:intersectionOf (
			rdf:List
			[
				rdf:type owl:Restriction ;
				owl:onProperty rdf:first ;
				owl:allValuesFrom mms-class:InRef ;
			]
			[
				rdf:type owl:Restriction ;
				owl:onProperty rdf:rest ;
				owl:allValuesFrom mms-class:InRefsList ;
			]
		) ;
	] .

mms-derived-property:isSite a mms-ontology:DerivedDatatypeProperty ;
	mms-ontology:key "_isSite" ;
	rdfs:label "isSite" ;
	rdfs:comment "Based on the key '_isSite'"@en ;
	rdfs:domain mms-class:Element ;
	rdfs:range xsd:boolean ;
	mms-ontology:mappingDomain mms-class:Element .

mms-derived-property:modified a mms-ontology:DerivedDatatypeProperty ;
	mms-ontology:key "_modified" ;
	rdfs:label "modified" ;
	rdfs:comment "Based on the key '_modified'"@en ;
	rdfs:domain mms-class:Element ;
	rdfs:range xsd:dateTime ;
	mms-ontology:mappingDomain mms-class:Element .

mms-derived-property:modifier a mms-ontology:DerivedObjectProperty ;
	mms-ontology:key "_modifier" ;
	rdfs:label "modifier" ;
	rdfs:comment "The user who last modified this Element"@en ;
	rdfs:domain mms-class:Element ;
	mms-ontology:mappingDomain mms-class:Element ;
	rdfs:range mms-ontology:User .

mms-derived-property:project a mms-ontology:DerivedObjectProperty ;
	mms-ontology:key "_projectId" ;
	rdfs:label "project" ;
	rdfs:comment "Based on the derived property '_projectId'."@en ;
	rdfs:domain mms-class:Element ;
	rdfs:range mms-class:Project ;
	mms-ontology:mappingDomain mms-class:Element .

mms-derived-property:propertyPaths a mms-ontology:DerivedObjectProperty ;
	mms-ontology:key "_propertyPathIds" ;
	rdfs:label "propertyPath" ;
	rdfs:comment "List of PropertyPaths that belong to this Element. Based on the derived property '_propertyPathIds'."@en ;
	rdfs:domain mms-class:Element ;
	rdfs:range mms-class:PropertyPathsList ;
	mms-ontology:listItemRange mms-class:PropertyPath ;
	mms-ontology:mappingDomain mms-class:Element .

mms-class:PropertyPathsList a owl:Class ;
	mms-ontology:category mms-class:ElementList ;
	rdfs:subClassOf [
		rdf:type owl:Class ;
		owl:intersectionOf (
			rdf:List
			[
				rdf:type owl:Restriction ;
				owl:onProperty rdf:first ;
				owl:allValuesFrom mms-class:PropertyPath ;
			]
			[
				rdf:type owl:Restriction ;
				owl:onProperty rdf:rest ;
				owl:allValuesFrom mms-class:PropertyPathsList ;
			]
		) ;
	] .

mms-derived-property:qualified a mms-ontology:DerivedObjectProperty ;
	mms-ontology:key "_qualifiedId" ;
	rdfs:label "qualified" ;
	rdfs:comment "Based on the derived property '_qualifiedId'."@en ;
	rdfs:domain mms-class:Element ;
	rdfs:range mms-class:Qualified ;
	mms-ontology:mappingDomain mms-class:Element .

mms-derived-property:ref a mms-ontology:DerivedObjectProperty ;
	mms-ontology:key "_refId" ;
	rdfs:label "ref" ;
	rdfs:comment "Based on the derived property '_refId'."@en ;
	rdfs:domain mms-class:Element ;
	rdfs:range mms-class:Ref ;
	mms-ontology:mappingDomain mms-class:Element .

mms-derived-property:sources a mms-ontology:DerivedObjectProperty ;
	mms-ontology:key "_sourceIds" ;
	rdfs:label "source" ;
	rdfs:comment "List of Sources that belong to this Element. Based on the derived property '_sourceIds'."@en ;
	rdfs:domain mms-class:Element ;
	rdfs:range mms-class:SourcesList ;
	mms-ontology:listItemRange mms-class:Source ;
	mms-ontology:mappingDomain mms-class:Element .

mms-class:SourcesList a owl:Class ;
	mms-ontology:category mms-class:ElementList ;
	rdfs:subClassOf [
		rdf:type owl:Class ;
		owl:intersectionOf (
			rdf:List
			[
				rdf:type owl:Restriction ;
				owl:onProperty rdf:first ;
				owl:allValuesFrom mms-class:Source ;
			]
			[
				rdf:type owl:Restriction ;
				owl:onProperty rdf:rest ;
				owl:allValuesFrom mms-class:SourcesList ;
			]
		) ;
	] .

mms-derived-property:targets a mms-ontology:DerivedObjectProperty ;
	mms-ontology:key "_targetIds" ;
	rdfs:label "target" ;
	rdfs:comment "List of Targets that belong to this Element. Based on the derived property '_targetIds'."@en ;
	rdfs:domain mms-class:Element ;
	rdfs:range mms-class:TargetsList ;
	mms-ontology:listItemRange mms-class:Target ;
	mms-ontology:mappingDomain mms-class:Element .

mms-class:TargetsList a owl:Class ;
	mms-ontology:category mms-class:ElementList ;
	rdfs:subClassOf [
		rdf:type owl:Class ;
		owl:intersectionOf (
			rdf:List
			[
				rdf:type owl:Restriction ;
				owl:onProperty rdf:first ;
				owl:allValuesFrom mms-class:Target ;
			]
			[
				rdf:type owl:Restriction ;
				owl:onProperty rdf:rest ;
				owl:allValuesFrom mms-class:TargetsList ;
			]
		) ;
	] .

mms-derived-property:veNumber a mms-ontology:DerivedDatatypeProperty ;
	mms-ontology:key "_veNumber" ;
	rdfs:label "veNumber" ;
	rdfs:comment "Based on the key '_veNumber'"@en ;
	rdfs:domain mms-class:Element ;
	rdfs:range xsd:string ;
	mms-ontology:mappingDomain mms-class:Element .

mms-property:activityFromActivityEdge a mms-ontology:UmlObjectProperty ;
	mms-ontology:key "activityId" ;
	rdfs:label "activityFromActivityEdge" ;
	rdfs:comment "The Activity that belongs to this ActivityEdge. Based on the UML property 'ActivityEdge-activity' which is described as: The Activity containing the ActivityEdge, if it is directly owned by an Activity.."@en ;
	rdfs:domain uml-class:ActivityEdge ;
	rdfs:range uml-class:Activity ;
	mms-ontology:umlPropertySource uml-property:ActivityEdge-activity .

mms-property:activityFromActivityNode a mms-ontology:UmlObjectProperty ;
	mms-ontology:key "activityId" ;
	rdfs:label "activityFromActivityNode" ;
	rdfs:comment "The Activity that belongs to this ActivityNode. Based on the UML property 'ActivityNode-activity' which is described as: The Activity containing the ActivityNode, if it is directly owned by an Activity.."@en ;
	rdfs:domain uml-class:ActivityNode ;
	rdfs:range uml-class:Activity ;
	mms-ontology:umlPropertySource uml-property:ActivityNode-activity .

mms-property:activityFromStructuredActivityNode a mms-ontology:UmlObjectProperty ;
	mms-ontology:key "activityId" ;
	rdfs:label "activityFromStructuredActivityNode" ;
	rdfs:comment "The Activity that belongs to this StructuredActivityNode. Based on the UML property 'StructuredActivityNode-activity' which is described as: The Activity immediately containing the StructuredActivityNode, if it is not contained in another StructuredActivityNode.."@en ;
	rdfs:domain uml-class:StructuredActivityNode ;
	rdfs:range uml-class:Activity ;
	mms-ontology:umlPropertySource uml-property:StructuredActivityNode-activity .

mms-property:additionUseCase a mms-ontology:UmlObjectProperty ;
	mms-ontology:key "additionId" ;
	rdfs:label "additionUseCase" ;
	rdfs:comment "The UseCase that is the addition of this Include. Based on the UML property 'Include-addition' which is described as: The UseCase that is to be included.."@en ;
	rdfs:domain uml-class:Include ;
	rdfs:range uml-class:UseCase ;
	mms-ontology:umlPropertySource uml-property:Include-addition .

mms-property:annotatedElement a mms-ontology:UmlObjectProperty ;
	mms-ontology:key "annotatedElementIds" ;
	rdfs:label "annotatedElement" ;
	rdfs:comment "A Element that belongs to this Comment. Based on the UML property 'Comment-annotatedElement' which is described as: References the Element(s) being commented.."@en ;
	rdfs:domain uml-class:Comment ;
	rdfs:range uml-class:Element ;
	mms-ontology:umlPropertySource uml-property:Comment-annotatedElement .

mms-property:appliedProfile a mms-ontology:UmlObjectProperty ;
	mms-ontology:key "appliedProfileId" ;
	rdfs:label "appliedProfile" ;
	rdfs:comment "The Profile that belongs to this ProfileApplication. Based on the UML property 'ProfileApplication-appliedProfile' which is described as: References the Profiles that are applied to a Package through this ProfileApplication.."@en ;
	rdfs:domain uml-class:ProfileApplication ;
	rdfs:range uml-class:Profile ;
	mms-ontology:umlPropertySource uml-property:ProfileApplication-appliedProfile .

mms-property:applyingPackage a mms-ontology:UmlObjectProperty ;
	mms-ontology:key "applyingPackageId" ;
	rdfs:label "applyingPackage" ;
	rdfs:comment "The Package that belongs to this ProfileApplication. Based on the UML property 'ProfileApplication-applyingPackage' which is described as: The package that owns the profile application.."@en ;
	rdfs:domain uml-class:ProfileApplication ;
	rdfs:range uml-class:Package ;
	mms-ontology:umlPropertySource uml-property:ProfileApplication-applyingPackage .

mms-property:argumentInputPin a mms-ontology:UmlObjectProperty ;
	mms-ontology:key "argumentIds" ;
	rdfs:label "argumentInputPin" ;
	rdfs:comment "A InputPin that is the argument of this InvocationAction. Based on the UML property 'InvocationAction-argument' which is described as: The InputPins that provide the argument values passed in the invocation request.."@en ;
	rdfs:domain uml-class:InvocationAction ;
	rdfs:range uml-class:InputPin ;
	mms-ontology:umlPropertySource uml-property:InvocationAction-argument .

mms-property:argumentValueSpecificationFromMessage a mms-ontology:UmlObjectProperty ;
	mms-ontology:key "argumentIds" ;
	rdfs:label "argumentValueSpecificationFromMessage" ;
	rdfs:comment "A ValueSpecification that is the argument of this Message. Based on the UML property 'Message-argument' which is described as: The arguments of the Message.."@en ;
	rdfs:domain uml-class:Message ;
	rdfs:range uml-class:ValueSpecification ;
	mms-ontology:umlPropertySource uml-property:Message-argument .

mms-property:argumentValueSpecificationFromInteractionUse a mms-ontology:UmlObjectProperty ;
	mms-ontology:key "argumentIds" ;
	rdfs:label "argumentValueSpecificationFromInteractionUse" ;
	rdfs:comment "A ValueSpecification that is the argument of this InteractionUse. Based on the UML property 'InteractionUse-argument' which is described as: The actual arguments of the Interaction.."@en ;
	rdfs:domain uml-class:InteractionUse ;
	rdfs:range uml-class:ValueSpecification ;
	mms-ontology:umlPropertySource uml-property:InteractionUse-argument .

mms-property:associationEndProperty a mms-ontology:UmlObjectProperty ;
	mms-ontology:key "associationEndId" ;
	rdfs:label "associationEndProperty" ;
	rdfs:comment "The Property that is the associationEnd of this Property. Based on the UML property 'Property-associationEnd' which is described as: Designates the optional association end that owns a qualifier attribute.."@en ;
	rdfs:domain uml-class:Property ;
	rdfs:range uml-class:Property ;
	mms-ontology:umlPropertySource uml-property:Property-associationEnd .

mms-property:associationFromProperty a mms-ontology:UmlObjectProperty ;
	mms-ontology:key "associationId" ;
	rdfs:label "associationFromProperty" ;
	rdfs:comment "The Association that belongs to this Property. Based on the UML property 'Property-association' which is described as: The Association of which this Property is a member, if any.."@en ;
	rdfs:domain uml-class:Property ;
	rdfs:range uml-class:Association ;
	mms-ontology:umlPropertySource uml-property:Property-association .

mms-property:associationFromClearAssociationAction a mms-ontology:UmlObjectProperty ;
	mms-ontology:key "associationId" ;
	rdfs:label "associationFromClearAssociationAction" ;
	rdfs:comment "The Association that belongs to this ClearAssociationAction. Based on the UML property 'ClearAssociationAction-association' which is described as: The Association to be cleared.."@en ;
	rdfs:domain uml-class:ClearAssociationAction ;
	rdfs:range uml-class:Association ;
	mms-ontology:umlPropertySource uml-property:ClearAssociationAction-association .

mms-property:behaviorFromBehaviorExecutionSpecification a mms-ontology:UmlObjectProperty ;
	mms-ontology:key "behaviorId" ;
	rdfs:label "behaviorFromBehaviorExecutionSpecification" ;
	rdfs:comment "The Behavior that belongs to this BehaviorExecutionSpecification. Based on the UML property 'BehaviorExecutionSpecification-behavior' which is described as: Behavior whose execution is occurring.."@en ;
	rdfs:domain uml-class:BehaviorExecutionSpecification ;
	rdfs:range uml-class:Behavior ;
	mms-ontology:umlPropertySource uml-property:BehaviorExecutionSpecification-behavior .

mms-property:behaviorFromOpaqueExpression a mms-ontology:UmlObjectProperty ;
	mms-ontology:key "behaviorId" ;
	rdfs:label "behaviorFromOpaqueExpression" ;
	rdfs:comment "The Behavior that belongs to this OpaqueExpression. Based on the UML property 'OpaqueExpression-behavior' which is described as: Specifies the behavior of the OpaqueExpression as a UML Behavior.."@en ;
	rdfs:domain uml-class:OpaqueExpression ;
	rdfs:range uml-class:Behavior ;
	mms-ontology:umlPropertySource uml-property:OpaqueExpression-behavior .

mms-property:behaviorFromCallBehaviorAction a mms-ontology:UmlObjectProperty ;
	mms-ontology:key "behaviorId" ;
	rdfs:label "behaviorFromCallBehaviorAction" ;
	rdfs:comment "The Behavior that belongs to this CallBehaviorAction. Based on the UML property 'CallBehaviorAction-behavior' which is described as: The Behavior being invoked.."@en ;
	rdfs:domain uml-class:CallBehaviorAction ;
	rdfs:range uml-class:Behavior ;
	mms-ontology:umlPropertySource uml-property:CallBehaviorAction-behavior .

mms-property:bodyPart a mms-ontology:UmlObjectProperty ;
	mms-ontology:key "bodyPartIds" ;
	rdfs:label "bodyPart" ;
	rdfs:comment "A ExecutableNode that is the bodyPart of this LoopNode. Based on the UML property 'LoopNode-bodyPart' which is described as: The set of ExecutableNodes that perform the repetitive computations of the loop. The bodyPart is executed as long as the test section produces a true value.."@en ;
	rdfs:domain uml-class:LoopNode ;
	rdfs:range uml-class:ExecutableNode ;
	mms-ontology:umlPropertySource uml-property:LoopNode-bodyPart .

mms-property:classifierBehavior a mms-ontology:UmlObjectProperty ;
	mms-ontology:key "classifierBehaviorId" ;
	rdfs:label "classifierBehavior" ;
	rdfs:comment "The Behavior that belongs to this BehavioredClassifier. Based on the UML property 'BehavioredClassifier-classifierBehavior' which is described as: A Behavior that specifies the behavior of the BehavioredClassifier itself.."@en ;
	rdfs:domain uml-class:BehavioredClassifier ;
	rdfs:range uml-class:Behavior ;
	mms-ontology:umlPropertySource uml-property:BehavioredClassifier-classifierBehavior .

mms-property:classifierFromReadIsClassifiedObjectAction a mms-ontology:UmlObjectProperty ;
	mms-ontology:key "classifierIds" ;
	rdfs:label "classifierFromReadIsClassifiedObjectAction" ;
	rdfs:comment "The Classifier that belongs to this ReadIsClassifiedObjectAction. Based on the UML property 'ReadIsClassifiedObjectAction-classifier' which is described as: The Classifier against which the classification of the input object is tested.."@en ;
	rdfs:domain uml-class:ReadIsClassifiedObjectAction ;
	rdfs:range uml-class:Classifier ;
	mms-ontology:umlPropertySource uml-property:ReadIsClassifiedObjectAction-classifier .

mms-property:classifierFromReadExtentAction a mms-ontology:UmlObjectProperty ;
	mms-ontology:key "classifierIds" ;
	rdfs:label "classifierFromReadExtentAction" ;
	rdfs:comment "The Classifier that belongs to this ReadExtentAction. Based on the UML property 'ReadExtentAction-classifier' which is described as: The Classifier whose instances are to be retrieved.."@en ;
	rdfs:domain uml-class:ReadExtentAction ;
	rdfs:range uml-class:Classifier ;
	mms-ontology:umlPropertySource uml-property:ReadExtentAction-classifier .

mms-property:classifierFromRedefinableTemplateSignature a mms-ontology:UmlObjectProperty ;
	mms-ontology:key "classifierIds" ;
	rdfs:label "classifierFromRedefinableTemplateSignature" ;
	rdfs:comment "The Classifier that belongs to this RedefinableTemplateSignature. Based on the UML property 'RedefinableTemplateSignature-classifier' which is described as: The Classifier that owns this RedefinableTemplateSignature.."@en ;
	rdfs:domain uml-class:RedefinableTemplateSignature ;
	rdfs:range uml-class:Classifier ;
	mms-ontology:umlPropertySource uml-property:RedefinableTemplateSignature-classifier .

mms-property:classifierFromCreateObjectAction a mms-ontology:UmlObjectProperty ;
	mms-ontology:key "classifierIds" ;
	rdfs:label "classifierFromCreateObjectAction" ;
	rdfs:comment "The Classifier that belongs to this CreateObjectAction. Based on the UML property 'CreateObjectAction-classifier' which is described as: The Classifier to be instantiated.."@en ;
	rdfs:domain uml-class:CreateObjectAction ;
	rdfs:range uml-class:Classifier ;
	mms-ontology:umlPropertySource uml-property:CreateObjectAction-classifier .

mms-property:classifierFromInstanceSpecification a mms-ontology:UmlObjectProperty ;
	mms-ontology:key "classifierIds" ;
	rdfs:label "classifierFromInstanceSpecification" ;
	rdfs:comment "A Classifier that belongs to this InstanceSpecification. Based on the UML property 'InstanceSpecification-classifier' which is described as: The Classifier or Classifiers of the represented instance. If multiple Classifiers are specified, the instance is classified by all of them.."@en ;
	rdfs:domain uml-class:InstanceSpecification ;
	rdfs:range uml-class:Classifier ;
	mms-ontology:umlPropertySource uml-property:InstanceSpecification-classifier .

mms-property:classifierEnumeration a mms-ontology:UmlObjectProperty ;
	mms-ontology:key "classifierIds" ;
	rdfs:label "classifierEnumeration" ;
	rdfs:comment "The Enumeration that is the classifier of this EnumerationLiteral. Based on the UML property 'EnumerationLiteral-classifier' which is described as: The classifier of this EnumerationLiteral derived to be equal to its Enumeration.."@en ;
	rdfs:domain uml-class:EnumerationLiteral ;
	rdfs:range uml-class:Enumeration ;
	mms-ontology:umlPropertySource uml-property:EnumerationLiteral-classifier .

mms-property:clientDependency a mms-ontology:UmlObjectProperty ;
	mms-ontology:key "clientDependencyIds" ;
	rdfs:label "clientDependency" ;
	rdfs:comment "A Dependency that belongs to this NamedElement. Based on the UML property 'NamedElement-clientDependency' which is described as: Indicates the Dependencies that reference this NamedElement as a client.."@en ;
	rdfs:domain uml-class:NamedElement ;
	rdfs:range uml-class:Dependency ;
	mms-ontology:umlPropertySource uml-property:NamedElement-clientDependency .

mms-property:client a mms-ontology:UmlObjectProperty ;
	mms-ontology:key "clientIds" ;
	rdfs:label "client" ;
	rdfs:comment "A NamedElement that is the client of this Dependency. Based on the UML property 'Dependency-client' which is described as: The Element(s) dependent on the supplier Element(s). In some cases (such as a trace Abstraction) the assignment of direction (that is, the designation of the client Element) is at the discretion of the modeler and is a stipulation.."@en ;
	rdfs:domain uml-class:Dependency ;
	rdfs:range uml-class:NamedElement ;
	mms-ontology:umlPropertySource uml-property:Dependency-client .

mms-property:constrainedElement a mms-ontology:UmlObjectProperty ;
	mms-ontology:key "constrainedElementIds" ;
	rdfs:label "constrainedElement" ;
	rdfs:comment "A Element that belongs to this Constraint. Based on the UML property 'Constraint-constrainedElement' which is described as: The ordered set of Elements referenced by this Constraint.."@en ;
	rdfs:domain uml-class:Constraint ;
	rdfs:range uml-class:Element ;
	mms-ontology:umlPropertySource uml-property:Constraint-constrainedElement .

mms-property:containerRegionFromTransition a mms-ontology:UmlObjectProperty ;
	mms-ontology:key "containerId" ;
	rdfs:label "containerRegionFromTransition" ;
	rdfs:comment "The Region that is the container of this Transition. Based on the UML property 'Transition-container' which is described as: Designates the Region that owns this Transition.."@en ;
	rdfs:domain uml-class:Transition ;
	rdfs:range uml-class:Region ;
	mms-ontology:umlPropertySource uml-property:Transition-container .

mms-property:containerRegionFromVertex a mms-ontology:UmlObjectProperty ;
	mms-ontology:key "containerId" ;
	rdfs:label "containerRegionFromVertex" ;
	rdfs:comment "The Region that is the container of this Vertex. Based on the UML property 'Vertex-container' which is described as: The Region that contains this Vertex.."@en ;
	rdfs:domain uml-class:Vertex ;
	rdfs:range uml-class:Region ;
	mms-ontology:umlPropertySource uml-property:Vertex-container .

mms-property:contextClassifier a mms-ontology:UmlObjectProperty ;
	mms-ontology:key "contextId" ;
	rdfs:label "contextClassifier" ;
	rdfs:comment "The Classifier that is the context of this Action. Based on the UML property 'Action-context' which is described as: The context Classifier of the Behavior that contains this Action, or the Behavior itself if it has no context.."@en ;
	rdfs:domain uml-class:Action ;
	rdfs:range uml-class:Classifier ;
	mms-ontology:umlPropertySource uml-property:Action-context .

mms-property:contextBehavioredClassifier a mms-ontology:UmlObjectProperty ;
	mms-ontology:key "contextId" ;
	rdfs:label "contextBehavioredClassifier" ;
	rdfs:comment "The BehavioredClassifier that is the context of this Behavior. Based on the UML property 'Behavior-context' which is described as: The BehavioredClassifier that is the context for the execution of the Behavior. A Behavior that is directly owned as a nestedClassifier does not have a context. Otherwise, to determine the context of a Behavior, find the first BehavioredClassifier reached by following the chain of owner relationships from the Behavior, if any. If there is such a BehavioredClassifier, then it is the context, unless it is itself a Behavior with a non-empty context, in which case that is also the context for the original Behavior. For example, following this algorithm, the context of an entry Behavior in a StateMachine is the BehavioredClassifier that owns the StateMachine. The features of the context BehavioredClassifier as well as the Elements visible to the context Classifier are visible to the Behavior.."@en ;
	rdfs:domain uml-class:Behavior ;
	rdfs:range uml-class:BehavioredClassifier ;
	mms-ontology:umlPropertySource uml-property:Behavior-context .

mms-property:contextNamespace a mms-ontology:UmlObjectProperty ;
	mms-ontology:key "contextId" ;
	rdfs:label "contextNamespace" ;
	rdfs:comment "The Namespace that is the context of this Constraint. Based on the UML property 'Constraint-context' which is described as: Specifies the Namespace that owns the Constraint.."@en ;
	rdfs:domain uml-class:Constraint ;
	rdfs:range uml-class:Namespace ;
	mms-ontology:umlPropertySource uml-property:Constraint-context .

mms-property:contractInterface a mms-ontology:UmlObjectProperty ;
	mms-ontology:key "contractId" ;
	rdfs:label "contractInterface" ;
	rdfs:comment "The Interface that is the contract of this InterfaceRealization. Based on the UML property 'InterfaceRealization-contract' which is described as: References the Interface specifying the conformance contract.."@en ;
	rdfs:domain uml-class:InterfaceRealization ;
	rdfs:range uml-class:Interface ;
	mms-ontology:umlPropertySource uml-property:InterfaceRealization-contract .

mms-property:contractBehavior a mms-ontology:UmlObjectProperty ;
	mms-ontology:key "contractId" ;
	rdfs:label "contractBehavior" ;
	rdfs:comment "The Behavior that is the contract of this Connector. Based on the UML property 'Connector-contract' which is described as: The set of Behaviors that specify the valid interaction patterns across the Connector.."@en ;
	rdfs:domain uml-class:Connector ;
	rdfs:range uml-class:Behavior ;
	mms-ontology:umlPropertySource uml-property:Connector-contract .

mms-property:contractClassifier a mms-ontology:UmlObjectProperty ;
	mms-ontology:key "contractId" ;
	rdfs:label "contractClassifier" ;
	rdfs:comment "The Classifier that is the contract of this Substitution. Based on the UML property 'Substitution-contract' which is described as: The contract with which the substituting classifier complies.."@en ;
	rdfs:domain uml-class:Substitution ;
	rdfs:range uml-class:Classifier ;
	mms-ontology:umlPropertySource uml-property:Substitution-contract .

mms-property:coveredBy a mms-ontology:UmlObjectProperty ;
	mms-ontology:key "coveredByIds" ;
	rdfs:label "coveredBy" ;
	rdfs:comment "A InteractionFragment that is the coveredBy of this Lifeline. Based on the UML property 'Lifeline-coveredBy' which is described as: References the InteractionFragments in which this Lifeline takes part.."@en ;
	rdfs:domain uml-class:Lifeline ;
	rdfs:range uml-class:InteractionFragment ;
	mms-ontology:umlPropertySource uml-property:Lifeline-coveredBy .

mms-property:coveredLifelineFromOccurrenceSpecification a mms-ontology:UmlObjectProperty ;
	mms-ontology:key "coveredIds" ;
	rdfs:label "coveredLifelineFromOccurrenceSpecification" ;
	rdfs:comment "The Lifeline that is the covered of this OccurrenceSpecification. Based on the UML property 'OccurrenceSpecification-covered' which is described as: References the Lifeline on which the OccurrenceSpecification appears.."@en ;
	rdfs:domain uml-class:OccurrenceSpecification ;
	rdfs:range uml-class:Lifeline ;
	mms-ontology:umlPropertySource uml-property:OccurrenceSpecification-covered .

mms-property:coveredFromInteractionFragment a mms-ontology:UmlObjectProperty ;
	mms-ontology:key "coveredIds" ;
	rdfs:label "coveredFromInteractionFragment" ;
	rdfs:comment "A Lifeline that is the covered of this InteractionFragment. Based on the UML property 'InteractionFragment-covered' which is described as: References the Lifelines that the InteractionFragment involves.."@en ;
	rdfs:domain uml-class:InteractionFragment ;
	rdfs:range uml-class:Lifeline ;
	mms-ontology:umlPropertySource uml-property:InteractionFragment-covered .

mms-property:coveredLifelineFromStateInvariant a mms-ontology:UmlObjectProperty ;
	mms-ontology:key "coveredIds" ;
	rdfs:label "coveredLifelineFromStateInvariant" ;
	rdfs:comment "The Lifeline that is the covered of this StateInvariant. Based on the UML property 'StateInvariant-covered' which is described as: References the Lifeline on which the StateInvariant appears.."@en ;
	rdfs:domain uml-class:StateInvariant ;
	rdfs:range uml-class:Lifeline ;
	mms-ontology:umlPropertySource uml-property:StateInvariant-covered .

mms-property:datatypeFromOperation a mms-ontology:UmlObjectProperty ;
	mms-ontology:key "datatypeId" ;
	rdfs:label "datatypeFromOperation" ;
	rdfs:comment "The DataType that belongs to this Operation. Based on the UML property 'Operation-datatype' which is described as: The DataType that owns this Operation, if any.."@en ;
	rdfs:domain uml-class:Operation ;
	rdfs:range uml-class:DataType ;
	mms-ontology:umlPropertySource uml-property:Operation-datatype .

mms-property:datatypeFromProperty a mms-ontology:UmlObjectProperty ;
	mms-ontology:key "datatypeId" ;
	rdfs:label "datatypeFromProperty" ;
	rdfs:comment "The DataType that belongs to this Property. Based on the UML property 'Property-datatype' which is described as: The DataType that owns this Property, if any.."@en ;
	rdfs:domain uml-class:Property ;
	rdfs:range uml-class:DataType ;
	mms-ontology:umlPropertySource uml-property:Property-datatype .

mms-property:deferrableTrigger a mms-ontology:UmlObjectProperty ;
	mms-ontology:key "deferrableTriggerIds" ;
	rdfs:label "deferrableTrigger" ;
	rdfs:comment "A Trigger that belongs to this State. Based on the UML property 'State-deferrableTrigger' which is described as: A list of Triggers that are candidates to be retained by the StateMachine if they trigger no Transitions out of the State (not consumed). A deferred Trigger is retained until the StateMachine reaches a State configuration where it is no longer deferred.."@en ;
	rdfs:domain uml-class:State ;
	rdfs:range uml-class:Trigger ;
	mms-ontology:umlPropertySource uml-property:State-deferrableTrigger .

mms-property:definingFeatureStructuralFeature a mms-ontology:UmlObjectProperty ;
	mms-ontology:key "definingFeatureId" ;
	rdfs:label "definingFeatureStructuralFeature" ;
	rdfs:comment "The StructuralFeature that is the definingFeature of this Slot. Based on the UML property 'Slot-definingFeature' which is described as: The StructuralFeature that specifies the values that may be held by the Slot.."@en ;
	rdfs:domain uml-class:Slot ;
	rdfs:range uml-class:StructuralFeature ;
	mms-ontology:umlPropertySource uml-property:Slot-definingFeature .

mms-property:doActivityBehavior a mms-ontology:UmlObjectProperty ;
	mms-ontology:key "doActivityId" ;
	rdfs:label "doActivityBehavior" ;
	rdfs:comment "The Behavior that is the doActivity of this State. Based on the UML property 'State-doActivity' which is described as: An optional Behavior that is executed while being in the State. The execution starts when this State is entered, and ceases either by itself when done, or when the State is exited, whichever comes first.."@en ;
	rdfs:domain uml-class:State ;
	rdfs:range uml-class:Behavior ;
	mms-ontology:umlPropertySource uml-property:State-doActivity .

mms-property:edgeFromActivity a mms-ontology:UmlObjectProperty ;
	mms-ontology:key "edgeIds" ;
	rdfs:label "edgeFromActivity" ;
	rdfs:comment "A ActivityEdge that is the edge of this Activity. Based on the UML property 'Activity-edge' which is described as: ActivityEdges expressing flow between the nodes of the Activity.."@en ;
	rdfs:domain uml-class:Activity ;
	rdfs:range uml-class:ActivityEdge ;
	mms-ontology:umlPropertySource uml-property:Activity-edge .

mms-property:edgeFromStructuredActivityNode a mms-ontology:UmlObjectProperty ;
	mms-ontology:key "edgeIds" ;
	rdfs:label "edgeFromStructuredActivityNode" ;
	rdfs:comment "A ActivityEdge that is the edge of this StructuredActivityNode. Based on the UML property 'StructuredActivityNode-edge' which is described as: The ActivityEdges immediately contained in the StructuredActivityNode.."@en ;
	rdfs:domain uml-class:StructuredActivityNode ;
	rdfs:range uml-class:ActivityEdge ;
	mms-ontology:umlPropertySource uml-property:StructuredActivityNode-edge .

mms-property:edgeFromActivityPartition a mms-ontology:UmlObjectProperty ;
	mms-ontology:key "edgeIds" ;
	rdfs:label "edgeFromActivityPartition" ;
	rdfs:comment "A ActivityEdge that is the edge of this ActivityPartition. Based on the UML property 'ActivityPartition-edge' which is described as: ActivityEdges immediately contained in the ActivityPartition.."@en ;
	rdfs:domain uml-class:ActivityPartition ;
	rdfs:range uml-class:ActivityEdge ;
	mms-ontology:umlPropertySource uml-property:ActivityPartition-edge .

mms-property:effectBehavior a mms-ontology:UmlObjectProperty ;
	mms-ontology:key "effectId" ;
	rdfs:label "effectBehavior" ;
	rdfs:comment "The Behavior that is the effect of this Transition. Based on the UML property 'Transition-effect' which is described as: Specifies an optional behavior to be performed when the Transition fires.."@en ;
	rdfs:domain uml-class:Transition ;
	rdfs:range uml-class:Behavior ;
	mms-ontology:umlPropertySource uml-property:Transition-effect .

mms-property:enclosingInteraction a mms-ontology:UmlObjectProperty ;
	mms-ontology:key "enclosingInteractionId" ;
	rdfs:label "enclosingInteraction" ;
	rdfs:comment "The Interaction that belongs to this InteractionFragment. Based on the UML property 'InteractionFragment-enclosingInteraction' which is described as: The Interaction enclosing this InteractionFragment.."@en ;
	rdfs:domain uml-class:InteractionFragment ;
	rdfs:range uml-class:Interaction ;
	mms-ontology:umlPropertySource uml-property:InteractionFragment-enclosingInteraction .

mms-property:endPropertyFromLinkEndData a mms-ontology:UmlObjectProperty ;
	mms-ontology:key "endIds" ;
	rdfs:label "endPropertyFromLinkEndData" ;
	rdfs:comment "The Property that is the end of this LinkEndData. Based on the UML property 'LinkEndData-end' which is described as: The Association end for which this LinkEndData specifies values.."@en ;
	rdfs:domain uml-class:LinkEndData ;
	rdfs:range uml-class:Property ;
	mms-ontology:umlPropertySource uml-property:LinkEndData-end .

mms-property:endPropertyFromReadLinkObjectEndAction a mms-ontology:UmlObjectProperty ;
	mms-ontology:key "endIds" ;
	rdfs:label "endPropertyFromReadLinkObjectEndAction" ;
	rdfs:comment "The Property that is the end of this ReadLinkObjectEndAction. Based on the UML property 'ReadLinkObjectEndAction-end' which is described as: The Association end to be read.."@en ;
	rdfs:domain uml-class:ReadLinkObjectEndAction ;
	rdfs:range uml-class:Property ;
	mms-ontology:umlPropertySource uml-property:ReadLinkObjectEndAction-end .

mms-property:endConnectorEndFromConnector a mms-ontology:UmlObjectProperty ;
	mms-ontology:key "endIds" ;
	rdfs:label "endConnectorEndFromConnector" ;
	rdfs:comment "A ConnectorEnd that is the end of this Connector. Based on the UML property 'Connector-end' which is described as: A Connector has at least two ConnectorEnds, each representing the participation of instances of the Classifiers typing the ConnectableElements attached to the end. The set of ConnectorEnds is ordered.."@en ;
	rdfs:domain uml-class:Connector ;
	rdfs:range uml-class:ConnectorEnd ;
	mms-ontology:umlPropertySource uml-property:Connector-end .

mms-property:endConnectorEndFromConnectableElement a mms-ontology:UmlObjectProperty ;
	mms-ontology:key "endIds" ;
	rdfs:label "endConnectorEndFromConnectableElement" ;
	rdfs:comment "A ConnectorEnd that is the end of this ConnectableElement. Based on the UML property 'ConnectableElement-end' which is described as: A set of ConnectorEnds that attach to this ConnectableElement.."@en ;
	rdfs:domain uml-class:ConnectableElement ;
	rdfs:range uml-class:ConnectorEnd ;
	mms-ontology:umlPropertySource uml-property:ConnectableElement-end .

mms-property:entryPseudostate a mms-ontology:UmlObjectProperty ;
	mms-ontology:key "entryId" ;
	rdfs:label "entryPseudostate" ;
	rdfs:comment "The Pseudostate that is the entry of this ConnectionPointReference. Based on the UML property 'ConnectionPointReference-entry' which is described as: The entryPoint Pseudostates corresponding to this connection point.."@en ;
	rdfs:domain uml-class:ConnectionPointReference ;
	rdfs:range uml-class:Pseudostate ;
	mms-ontology:umlPropertySource uml-property:ConnectionPointReference-entry .

mms-property:entryBehavior a mms-ontology:UmlObjectProperty ;
	mms-ontology:key "entryId" ;
	rdfs:label "entryBehavior" ;
	rdfs:comment "The Behavior that is the entry of this State. Based on the UML property 'State-entry' which is described as: An optional Behavior that is executed whenever this State is entered regardless of the Transition taken to reach the State. If defined, entry Behaviors are always executed to completion prior to any internal Behavior or Transitions performed within the State.."@en ;
	rdfs:domain uml-class:State ;
	rdfs:range uml-class:Behavior ;
	mms-ontology:umlPropertySource uml-property:State-entry .

mms-property:enumeration a mms-ontology:UmlObjectProperty ;
	mms-ontology:key "enumerationId" ;
	rdfs:label "enumeration" ;
	rdfs:comment "The Enumeration that belongs to this EnumerationLiteral. Based on the UML property 'EnumerationLiteral-enumeration' which is described as: The Enumeration that this EnumerationLiteral is a member of.."@en ;
	rdfs:domain uml-class:EnumerationLiteral ;
	rdfs:range uml-class:Enumeration ;
	mms-ontology:umlPropertySource uml-property:EnumerationLiteral-enumeration .

mms-property:eventNamedElementFromTimeObservation a mms-ontology:UmlObjectProperty ;
	mms-ontology:key "eventId" ;
	rdfs:label "eventNamedElementFromTimeObservation" ;
	rdfs:comment "The NamedElement that is the event of this TimeObservation. Based on the UML property 'TimeObservation-event' which is described as: The TimeObservation is determined by the entering or exiting of the event Element during execution.."@en ;
	rdfs:domain uml-class:TimeObservation ;
	rdfs:range uml-class:NamedElement ;
	mms-ontology:umlPropertySource uml-property:TimeObservation-event .

mms-property:eventNamedElementFromDurationObservation a mms-ontology:UmlObjectProperty ;
	mms-ontology:key "eventId" ;
	rdfs:label "eventNamedElementFromDurationObservation" ;
	rdfs:comment "The NamedElement that is the event of this DurationObservation. Based on the UML property 'DurationObservation-event' which is described as: The DurationObservation is determined as the duration between the entering or exiting of a single event Element during execution, or the entering/exiting of one event Element and the entering/exiting of a second.."@en ;
	rdfs:domain uml-class:DurationObservation ;
	rdfs:range uml-class:NamedElement ;
	mms-ontology:umlPropertySource uml-property:DurationObservation-event .

mms-property:event a mms-ontology:UmlObjectProperty ;
	mms-ontology:key "eventId" ;
	rdfs:label "event" ;
	rdfs:comment "The Event that belongs to this Trigger. Based on the UML property 'Trigger-event' which is described as: The Event that detected by the Trigger.."@en ;
	rdfs:domain uml-class:Trigger ;
	rdfs:range uml-class:Event ;
	mms-ontology:umlPropertySource uml-property:Trigger-event .

mms-property:eventNamedElementFromTimeObservation a mms-ontology:UmlObjectProperty ;
	mms-ontology:key "eventIds" ;
	rdfs:label "eventNamedElementFromTimeObservation" ;
	rdfs:comment "The NamedElement that is the event of this TimeObservation. Based on the UML property 'TimeObservation-event' which is described as: The TimeObservation is determined by the entering or exiting of the event Element during execution.."@en ;
	rdfs:domain uml-class:TimeObservation ;
	rdfs:range uml-class:NamedElement ;
	mms-ontology:umlPropertySource uml-property:TimeObservation-event .

mms-property:eventNamedElementsFromDurationObservation a mms-ontology:UmlObjectProperty ;
	mms-ontology:key "eventIds" ;
	rdfs:label "eventNamedElementsFromDurationObservation" ;
	rdfs:comment "List of NamedElements that are the event of this DurationObservation. Based on the UML property 'DurationObservation-event' which is described as: The DurationObservation is determined as the duration between the entering or exiting of a single event Element during execution, or the entering/exiting of one event Element and the entering/exiting of a second.."@en ;
	rdfs:domain uml-class:DurationObservation ;
	rdfs:range mms-class:EventNamedElementsFromDurationObservationList ;
	mms-ontology:listItemRange uml-class:NamedElement ;
	mms-ontology:umlPropertySource uml-property:DurationObservation-event .

mms-class:EventNamedElementsFromDurationObservationList a owl:Class ;
	mms-ontology:category mms-class:ElementList ;
	rdfs:subClassOf [
		rdf:type owl:Class ;
		owl:intersectionOf (
			rdf:List
			[
				rdf:type owl:Restriction ;
				owl:onProperty rdf:first ;
				owl:allValuesFrom uml-class:NamedElement ;
			]
			[
				rdf:type owl:Restriction ;
				owl:onProperty rdf:rest ;
				owl:allValuesFrom mms-class:EventNamedElementsFromDurationObservationList ;
			]
		) ;
	] .

mms-property:event a mms-ontology:UmlObjectProperty ;
	mms-ontology:key "eventIds" ;
	rdfs:label "event" ;
	rdfs:comment "The Event that belongs to this Trigger. Based on the UML property 'Trigger-event' which is described as: The Event that detected by the Trigger.."@en ;
	rdfs:domain uml-class:Trigger ;
	rdfs:range uml-class:Event ;
	mms-ontology:umlPropertySource uml-property:Trigger-event .

mms-property:exitPseudostate a mms-ontology:UmlObjectProperty ;
	mms-ontology:key "exitId" ;
	rdfs:label "exitPseudostate" ;
	rdfs:comment "The Pseudostate that is the exit of this ConnectionPointReference. Based on the UML property 'ConnectionPointReference-exit' which is described as: The exitPoints kind Pseudostates corresponding to this connection point.."@en ;
	rdfs:domain uml-class:ConnectionPointReference ;
	rdfs:range uml-class:Pseudostate ;
	mms-ontology:umlPropertySource uml-property:ConnectionPointReference-exit .

mms-property:exitBehavior a mms-ontology:UmlObjectProperty ;
	mms-ontology:key "exitId" ;
	rdfs:label "exitBehavior" ;
	rdfs:comment "The Behavior that is the exit of this State. Based on the UML property 'State-exit' which is described as: An optional Behavior that is executed whenever this State is exited regardless of which Transition was taken out of the State. If defined, exit Behaviors are always executed to completion only after all internal and transition Behaviors have completed execution.."@en ;
	rdfs:domain uml-class:State ;
	rdfs:range uml-class:Behavior ;
	mms-ontology:umlPropertySource uml-property:State-exit .

mms-property:fragmentFromInteraction a mms-ontology:UmlObjectProperty ;
	mms-ontology:key "fragmentIds" ;
	rdfs:label "fragmentFromInteraction" ;
	rdfs:comment "A InteractionFragment that is the fragment of this Interaction. Based on the UML property 'Interaction-fragment' which is described as: The ordered set of fragments in the Interaction.."@en ;
	rdfs:domain uml-class:Interaction ;
	rdfs:range uml-class:InteractionFragment ;
	mms-ontology:umlPropertySource uml-property:Interaction-fragment .

mms-property:fragmentFromInteractionOperand a mms-ontology:UmlObjectProperty ;
	mms-ontology:key "fragmentIds" ;
	rdfs:label "fragmentFromInteractionOperand" ;
	rdfs:comment "A InteractionFragment that is the fragment of this InteractionOperand. Based on the UML property 'InteractionOperand-fragment' which is described as: The fragments of the operand.."@en ;
	rdfs:domain uml-class:InteractionOperand ;
	rdfs:range uml-class:InteractionFragment ;
	mms-ontology:umlPropertySource uml-property:InteractionOperand-fragment .

mms-property:generalClassifierFromClassifier a mms-ontology:UmlObjectProperty ;
	mms-ontology:key "generalId" ;
	rdfs:label "generalClassifierFromClassifier" ;
	rdfs:comment "The Classifier that is the general of this Classifier. Based on the UML property 'Classifier-general' which is described as: The generalizing Classifiers for this Classifier.."@en ;
	rdfs:domain uml-class:Classifier ;
	rdfs:range uml-class:Classifier ;
	mms-ontology:umlPropertySource uml-property:Classifier-general .

mms-property:generalClassifierFromGeneralization a mms-ontology:UmlObjectProperty ;
	mms-ontology:key "generalId" ;
	rdfs:label "generalClassifierFromGeneralization" ;
	rdfs:comment "The Classifier that is the general of this Generalization. Based on the UML property 'Generalization-general' which is described as: The general classifier in the Generalization relationship.."@en ;
	rdfs:domain uml-class:Generalization ;
	rdfs:range uml-class:Classifier ;
	mms-ontology:umlPropertySource uml-property:Generalization-general .

mms-property:generalizationFromClassifier a mms-ontology:UmlObjectProperty ;
	mms-ontology:key "generalizationIds" ;
	rdfs:label "generalizationFromClassifier" ;
	rdfs:comment "A Generalization that belongs to this Classifier. Based on the UML property 'Classifier-generalization' which is described as: The Generalization relationships for this Classifier. These Generalizations navigate to more general Classifiers in the generalization hierarchy.."@en ;
	rdfs:domain uml-class:Classifier ;
	rdfs:range uml-class:Generalization ;
	mms-ontology:umlPropertySource uml-property:Classifier-generalization .

mms-property:generalizationFromGeneralizationSet a mms-ontology:UmlObjectProperty ;
	mms-ontology:key "generalizationIds" ;
	rdfs:label "generalizationFromGeneralizationSet" ;
	rdfs:comment "A Generalization that belongs to this GeneralizationSet. Based on the UML property 'GeneralizationSet-generalization' which is described as: Designates the instances of Generalization that are members of this GeneralizationSet.."@en ;
	rdfs:domain uml-class:GeneralizationSet ;
	rdfs:range uml-class:Generalization ;
	mms-ontology:umlPropertySource uml-property:GeneralizationSet-generalization .

mms-property:group a mms-ontology:UmlObjectProperty ;
	mms-ontology:key "groupIds" ;
	rdfs:label "group" ;
	rdfs:comment "A ActivityGroup that is the group of this Activity. Based on the UML property 'Activity-group' which is described as: Top-level ActivityGroups in the Activity.."@en ;
	rdfs:domain uml-class:Activity ;
	rdfs:range uml-class:ActivityGroup ;
	mms-ontology:umlPropertySource uml-property:Activity-group .

mms-property:guardConstraint a mms-ontology:UmlObjectProperty ;
	mms-ontology:key "guardId" ;
	rdfs:label "guardConstraint" ;
	rdfs:comment "The Constraint that is the guard of this Transition. Based on the UML property 'Transition-guard' which is described as: A guard is a Constraint that provides a fine-grained control over the firing of the Transition. The guard is evaluated when an Event occurrence is dispatched by the StateMachine. If the guard is true at that time, the Transition may be enabled, otherwise, it is disabled. Guards should be pure expressions without side effects. Guard expressions with side effects are ill formed.."@en ;
	rdfs:domain uml-class:Transition ;
	rdfs:range uml-class:Constraint ;
	mms-ontology:umlPropertySource uml-property:Transition-guard .

mms-property:guardValueSpecification a mms-ontology:UmlObjectProperty ;
	mms-ontology:key "guardId" ;
	rdfs:label "guardValueSpecification" ;
	rdfs:comment "The ValueSpecification that is the guard of this ActivityEdge. Based on the UML property 'ActivityEdge-guard' which is described as: A ValueSpecification that is evaluated to determine if a token can traverse the ActivityEdge. If an ActivityEdge has no guard, then there is no restriction on tokens traversing the edge.."@en ;
	rdfs:domain uml-class:ActivityEdge ;
	rdfs:range uml-class:ValueSpecification ;
	mms-ontology:umlPropertySource uml-property:ActivityEdge-guard .

mms-property:guardInteractionConstraint a mms-ontology:UmlObjectProperty ;
	mms-ontology:key "guardId" ;
	rdfs:label "guardInteractionConstraint" ;
	rdfs:comment "The InteractionConstraint that is the guard of this InteractionOperand. Based on the UML property 'InteractionOperand-guard' which is described as: Constraint of the operand.."@en ;
	rdfs:domain uml-class:InteractionOperand ;
	rdfs:range uml-class:InteractionConstraint ;
	mms-ontology:umlPropertySource uml-property:InteractionOperand-guard .

mms-property:implementingClassifierBehavioredClassifier a mms-ontology:UmlObjectProperty ;
	mms-ontology:key "implementingClassifierId" ;
	rdfs:label "implementingClassifierBehavioredClassifier" ;
	rdfs:comment "The BehavioredClassifier that is the implementingClassifier of this InterfaceRealization. Based on the UML property 'InterfaceRealization-implementingClassifier' which is described as: References the BehavioredClassifier that owns this InterfaceRealization, i.e., the BehavioredClassifier that realizes the Interface to which it refers.."@en ;
	rdfs:domain uml-class:InterfaceRealization ;
	rdfs:range uml-class:BehavioredClassifier ;
	mms-ontology:umlPropertySource uml-property:InterfaceRealization-implementingClassifier .

mms-property:importedPackage a mms-ontology:UmlObjectProperty ;
	mms-ontology:key "importedPackageId" ;
	rdfs:label "importedPackage" ;
	rdfs:comment "The Package that belongs to this PackageImport. Based on the UML property 'PackageImport-importedPackage' which is described as: Specifies the Package whose members are imported into a Namespace.."@en ;
	rdfs:domain uml-class:PackageImport ;
	rdfs:range uml-class:Package ;
	mms-ontology:umlPropertySource uml-property:PackageImport-importedPackage .

mms-property:importingNamespaceFromPackageImport a mms-ontology:UmlObjectProperty ;
	mms-ontology:key "importingNamespaceId" ;
	rdfs:label "importingNamespaceFromPackageImport" ;
	rdfs:comment "The Namespace that belongs to this PackageImport. Based on the UML property 'PackageImport-importingNamespace' which is described as: Specifies the Namespace that imports the members from a Package.."@en ;
	rdfs:domain uml-class:PackageImport ;
	rdfs:range uml-class:Namespace ;
	mms-ontology:umlPropertySource uml-property:PackageImport-importingNamespace .

mms-property:importingNamespaceFromElementImport a mms-ontology:UmlObjectProperty ;
	mms-ontology:key "importingNamespaceId" ;
	rdfs:label "importingNamespaceFromElementImport" ;
	rdfs:comment "The Namespace that belongs to this ElementImport. Based on the UML property 'ElementImport-importingNamespace' which is described as: Specifies the Namespace that imports a PackageableElement from another Namespace.."@en ;
	rdfs:domain uml-class:ElementImport ;
	rdfs:range uml-class:Namespace ;
	mms-ontology:umlPropertySource uml-property:ElementImport-importingNamespace .

mms-property:inActivity a mms-ontology:UmlObjectProperty ;
	mms-ontology:key "inActivityId" ;
	rdfs:label "inActivity" ;
	rdfs:comment "The Activity that belongs to this ActivityGroup. Based on the UML property 'ActivityGroup-inActivity' which is described as: The Activity containing the ActivityGroup, if it is directly owned by an Activity.."@en ;
	rdfs:domain uml-class:ActivityGroup ;
	rdfs:range uml-class:Activity ;
	mms-ontology:umlPropertySource uml-property:ActivityGroup-inActivity .

mms-property:inPartitionFromActivityNode a mms-ontology:UmlObjectProperty ;
	mms-ontology:key "inPartitionIds" ;
	rdfs:label "inPartitionFromActivityNode" ;
	rdfs:comment "A ActivityPartition that is the inPartition of this ActivityNode. Based on the UML property 'ActivityNode-inPartition' which is described as: ActivityPartitions containing the ActivityNode.."@en ;
	rdfs:domain uml-class:ActivityNode ;
	rdfs:range uml-class:ActivityPartition ;
	mms-ontology:umlPropertySource uml-property:ActivityNode-inPartition .

mms-property:inPartitionFromActivityEdge a mms-ontology:UmlObjectProperty ;
	mms-ontology:key "inPartitionIds" ;
	rdfs:label "inPartitionFromActivityEdge" ;
	rdfs:comment "A ActivityPartition that is the inPartition of this ActivityEdge. Based on the UML property 'ActivityEdge-inPartition' which is described as: ActivityPartitions containing the ActivityEdge.."@en ;
	rdfs:domain uml-class:ActivityEdge ;
	rdfs:range uml-class:ActivityPartition ;
	mms-ontology:umlPropertySource uml-property:ActivityEdge-inPartition .

mms-property:inStructuredNodeStructuredActivityNodeFromActivityNode a mms-ontology:UmlObjectProperty ;
	mms-ontology:key "inStructuredNodeId" ;
	rdfs:label "inStructuredNodeStructuredActivityNodeFromActivityNode" ;
	rdfs:comment "The StructuredActivityNode that is the inStructuredNode of this ActivityNode. Based on the UML property 'ActivityNode-inStructuredNode' which is described as: The StructuredActivityNode containing the ActvityNode, if it is directly owned by a StructuredActivityNode.."@en ;
	rdfs:domain uml-class:ActivityNode ;
	rdfs:range uml-class:StructuredActivityNode ;
	mms-ontology:umlPropertySource uml-property:ActivityNode-inStructuredNode .

mms-property:inStructuredNodeStructuredActivityNodeFromActivityEdge a mms-ontology:UmlObjectProperty ;
	mms-ontology:key "inStructuredNodeId" ;
	rdfs:label "inStructuredNodeStructuredActivityNodeFromActivityEdge" ;
	rdfs:comment "The StructuredActivityNode that is the inStructuredNode of this ActivityEdge. Based on the UML property 'ActivityEdge-inStructuredNode' which is described as: The StructuredActivityNode containing the ActivityEdge, if it is owned by a StructuredActivityNode.."@en ;
	rdfs:domain uml-class:ActivityEdge ;
	rdfs:range uml-class:StructuredActivityNode ;
	mms-ontology:umlPropertySource uml-property:ActivityEdge-inStructuredNode .

mms-property:include a mms-ontology:UmlObjectProperty ;
	mms-ontology:key "includeIds" ;
	rdfs:label "include" ;
	rdfs:comment "A Include that belongs to this UseCase. Based on the UML property 'UseCase-include' which is described as: The Include relationships owned by this UseCase.."@en ;
	rdfs:domain uml-class:UseCase ;
	rdfs:range uml-class:Include ;
	mms-ontology:umlPropertySource uml-property:UseCase-include .

mms-property:includingCaseUseCase a mms-ontology:UmlObjectProperty ;
	mms-ontology:key "includingCaseId" ;
	rdfs:label "includingCaseUseCase" ;
	rdfs:comment "The UseCase that is the includingCase of this Include. Based on the UML property 'Include-includingCase' which is described as: The UseCase which includes the addition and owns the Include relationship.."@en ;
	rdfs:domain uml-class:Include ;
	rdfs:range uml-class:UseCase ;
	mms-ontology:umlPropertySource uml-property:Include-includingCase .

mms-property:incomingActivityEdge a mms-ontology:UmlObjectProperty ;
	mms-ontology:key "incomingIds" ;
	rdfs:label "incomingActivityEdge" ;
	rdfs:comment "A ActivityEdge that is the incoming of this ActivityNode. Based on the UML property 'ActivityNode-incoming' which is described as: ActivityEdges that have the ActivityNode as their target.."@en ;
	rdfs:domain uml-class:ActivityNode ;
	rdfs:range uml-class:ActivityEdge ;
	mms-ontology:umlPropertySource uml-property:ActivityNode-incoming .

mms-property:incomingTransition a mms-ontology:UmlObjectProperty ;
	mms-ontology:key "incomingIds" ;
	rdfs:label "incomingTransition" ;
	rdfs:comment "A Transition that is the incoming of this Vertex. Based on the UML property 'Vertex-incoming' which is described as: Specifies the Transitions entering this Vertex.."@en ;
	rdfs:domain uml-class:Vertex ;
	rdfs:range uml-class:Transition ;
	mms-ontology:umlPropertySource uml-property:Vertex-incoming .

mms-property:informationSource a mms-ontology:UmlObjectProperty ;
	mms-ontology:key "informationSourceIds" ;
	rdfs:label "informationSource" ;
	rdfs:comment "A NamedElement that is the informationSource of this InformationFlow. Based on the UML property 'InformationFlow-informationSource' which is described as: Defines from which source the conveyed InformationItems are initiated.."@en ;
	rdfs:domain uml-class:InformationFlow ;
	rdfs:range uml-class:NamedElement ;
	mms-ontology:umlPropertySource uml-property:InformationFlow-informationSource .

mms-property:informationTarget a mms-ontology:UmlObjectProperty ;
	mms-ontology:key "informationTargetIds" ;
	rdfs:label "informationTarget" ;
	rdfs:comment "A NamedElement that is the informationTarget of this InformationFlow. Based on the UML property 'InformationFlow-informationTarget' which is described as: Defines to which target the conveyed InformationItems are directed.."@en ;
	rdfs:domain uml-class:InformationFlow ;
	rdfs:range uml-class:NamedElement ;
	mms-ontology:umlPropertySource uml-property:InformationFlow-informationTarget .

mms-property:inputElement a mms-ontology:UmlObjectProperty ;
	mms-ontology:key "inputElementIds" ;
	rdfs:label "inputElement" ;
	rdfs:comment "A ExpansionNode that is the inputElement of this ExpansionRegion. Based on the UML property 'ExpansionRegion-inputElement' which is described as: The ExpansionNodes that hold the input collections for the ExpansionRegion.."@en ;
	rdfs:domain uml-class:ExpansionRegion ;
	rdfs:range uml-class:ExpansionNode ;
	mms-ontology:umlPropertySource uml-property:ExpansionRegion-inputElement .

mms-property:inputValueFromOpaqueAction a mms-ontology:UmlObjectProperty ;
	mms-ontology:key "inputValueIds" ;
	rdfs:label "inputValueFromOpaqueAction" ;
	rdfs:comment "A InputPin that is the inputValue of this OpaqueAction. Based on the UML property 'OpaqueAction-inputValue' which is described as: The InputPins providing inputs to the OpaqueAction.."@en ;
	rdfs:domain uml-class:OpaqueAction ;
	rdfs:range uml-class:InputPin ;
	mms-ontology:umlPropertySource uml-property:OpaqueAction-inputValue .

mms-property:inputValueFromLinkAction a mms-ontology:UmlObjectProperty ;
	mms-ontology:key "inputValueIds" ;
	rdfs:label "inputValueFromLinkAction" ;
	rdfs:comment "A InputPin that is the inputValue of this LinkAction. Based on the UML property 'LinkAction-inputValue' which is described as: InputPins used by the LinkEndData of the LinkAction.."@en ;
	rdfs:domain uml-class:LinkAction ;
	rdfs:range uml-class:InputPin ;
	mms-ontology:umlPropertySource uml-property:LinkAction-inputValue .

mms-property:interactionFromLifeline a mms-ontology:UmlObjectProperty ;
	mms-ontology:key "interactionId" ;
	rdfs:label "interactionFromLifeline" ;
	rdfs:comment "The Interaction that belongs to this Lifeline. Based on the UML property 'Lifeline-interaction' which is described as: References the Interaction enclosing this Lifeline.."@en ;
	rdfs:domain uml-class:Lifeline ;
	rdfs:range uml-class:Interaction ;
	mms-ontology:umlPropertySource uml-property:Lifeline-interaction .

mms-property:interactionFromMessage a mms-ontology:UmlObjectProperty ;
	mms-ontology:key "interactionId" ;
	rdfs:label "interactionFromMessage" ;
	rdfs:comment "The Interaction that belongs to this Message. Based on the UML property 'Message-interaction' which is described as: The enclosing Interaction owning the Message.."@en ;
	rdfs:domain uml-class:Message ;
	rdfs:range uml-class:Interaction ;
	mms-ontology:umlPropertySource uml-property:Message-interaction .

mms-property:interfaceRealization a mms-ontology:UmlObjectProperty ;
	mms-ontology:key "interfaceRealizationIds" ;
	rdfs:label "interfaceRealization" ;
	rdfs:comment "A InterfaceRealization that belongs to this BehavioredClassifier. Based on the UML property 'BehavioredClassifier-interfaceRealization' which is described as: The set of InterfaceRealizations owned by the BehavioredClassifier. Interface realizations reference the Interfaces of which the BehavioredClassifier is an implementation.."@en ;
	rdfs:domain uml-class:BehavioredClassifier ;
	rdfs:range uml-class:InterfaceRealization ;
	mms-ontology:umlPropertySource uml-property:BehavioredClassifier-interfaceRealization .

mms-property:invariantConstraint a mms-ontology:UmlObjectProperty ;
	mms-ontology:key "invariantId" ;
	rdfs:label "invariantConstraint" ;
	rdfs:comment "The Constraint that is the invariant of this StateInvariant. Based on the UML property 'StateInvariant-invariant' which is described as: A Constraint that should hold at runtime for this StateInvariant.."@en ;
	rdfs:domain uml-class:StateInvariant ;
	rdfs:range uml-class:Constraint ;
	mms-ontology:umlPropertySource uml-property:StateInvariant-invariant .

mms-property:isAbstractBehavioralFeature a mms-ontology:UmlDatatypeProperty ;
	mms-ontology:key "isAbstract" ;
	rdfs:label "isAbstractBehavioralFeature" ;
	rdfs:comment "If true, then the BehavioralFeature does not have an implementation, and one must be supplied by a more specific Classifier. If false, the BehavioralFeature must have an implementation in the Classifier or one must be inherited."@en ;
	rdfs:domain uml-class:BehavioralFeature ;
	rdfs:range xsd:boolean ;
	mms-ontology:umlPropertySource uml-property:BehavioralFeature-isAbstract .

mms-property:isAbstractClassifier a mms-ontology:UmlDatatypeProperty ;
	mms-ontology:key "isAbstract" ;
	rdfs:label "isAbstractClassifier" ;
	rdfs:comment "If true, the Classifier can only be instantiated by instantiating one of its specializations. An abstract Classifier is intended to be used by other Classifiers e.g., as the target of Associations or Generalizations."@en ;
	rdfs:domain uml-class:Classifier ;
	rdfs:range xsd:boolean ;
	mms-ontology:umlPropertySource uml-property:Classifier-isAbstract .

mms-property:isAbstractClass a mms-ontology:UmlDatatypeProperty ;
	mms-ontology:key "isAbstract" ;
	rdfs:label "isAbstractClass" ;
	rdfs:comment "If true, the Class does not provide a complete declaration and cannot be instantiated. An abstract Class is typically used as a target of Associations or Generalizations."@en ;
	rdfs:domain uml-class:Class ;
	rdfs:range xsd:boolean ;
	mms-ontology:umlPropertySource uml-property:Class-isAbstract .

mms-property:isActive a mms-ontology:UmlDatatypeProperty ;
	mms-ontology:key "isActive" ;
	rdfs:label "isActive" ;
	rdfs:comment "Determines whether an object specified by this Class is active or not. If true, then the owning Class is referred to as an active Class. If false, then such a Class is referred to as a passive Class."@en ;
	rdfs:domain uml-class:Class ;
	rdfs:range xsd:boolean ;
	mms-ontology:umlPropertySource uml-property:Class-isActive .

mms-property:isActiveClass a mms-ontology:UmlDatatypeProperty ;
	owl:equivalentProperty mms-property:isActive .

mms-property:isBehavior a mms-ontology:UmlDatatypeProperty ;
	mms-ontology:key "isBehavior" ;
	rdfs:label "isBehavior" ;
	rdfs:comment "Specifies whether requests arriving at this Port are sent to the classifier behavior of this EncapsulatedClassifier. Such a Port is referred to as a behavior Port. Any invocation of a BehavioralFeature targeted at a behavior Port will be handled by the instance of the owning EncapsulatedClassifier itself, rather than by any instances that it may contain."@en ;
	rdfs:domain uml-class:Port ;
	rdfs:range xsd:boolean ;
	mms-ontology:umlPropertySource uml-property:Port-isBehavior .

mms-property:isBehaviorPort a mms-ontology:UmlDatatypeProperty ;
	owl:equivalentProperty mms-property:isBehavior .

mms-property:isCombineDuplicate a mms-ontology:UmlDatatypeProperty ;
	mms-ontology:key "isCombineDuplicate" ;
	rdfs:label "isCombineDuplicate" ;
	rdfs:comment "Indicates whether incoming tokens having objects with the same identity are combined into one by the JoinNode."@en ;
	rdfs:domain uml-class:JoinNode ;
	rdfs:range xsd:boolean ;
	mms-ontology:umlPropertySource uml-property:JoinNode-isCombineDuplicate .

mms-property:isCombineDuplicateJoinNode a mms-ontology:UmlDatatypeProperty ;
	owl:equivalentProperty mms-property:isCombineDuplicate .

mms-property:isConjugated a mms-ontology:UmlDatatypeProperty ;
	mms-ontology:key "isConjugated" ;
	rdfs:label "isConjugated" ;
	rdfs:comment "Specifies the way that the provided and required Interfaces are derived from the Port’s Type."@en ;
	rdfs:domain uml-class:Port ;
	rdfs:range xsd:boolean ;
	mms-ontology:umlPropertySource uml-property:Port-isConjugated .

mms-property:isConjugatedPort a mms-ontology:UmlDatatypeProperty ;
	owl:equivalentProperty mms-property:isConjugated .

mms-property:isControl a mms-ontology:UmlDatatypeProperty ;
	mms-ontology:key "isControl" ;
	rdfs:label "isControl" ;
	rdfs:comment "Indicates whether the Pin provides data to the Action or just controls how the Action executes."@en ;
	rdfs:domain uml-class:Pin ;
	rdfs:range xsd:boolean ;
	mms-ontology:umlPropertySource uml-property:Pin-isControl .

mms-property:isControlPin a mms-ontology:UmlDatatypeProperty ;
	owl:equivalentProperty mms-property:isControl .

mms-property:isControlType a mms-ontology:UmlDatatypeProperty ;
	mms-ontology:key "isControlType" ;
	rdfs:label "isControlType" ;
	rdfs:comment "Indicates whether the type of the ObjectNode is to be treated as representing control values that may traverse ControlFlows."@en ;
	rdfs:domain uml-class:ObjectNode ;
	rdfs:range xsd:boolean ;
	mms-ontology:umlPropertySource uml-property:ObjectNode-isControlType .

mms-property:isControlTypeObjectNode a mms-ontology:UmlDatatypeProperty ;
	owl:equivalentProperty mms-property:isControlType .

mms-property:isDerivedProperty a mms-ontology:UmlDatatypeProperty ;
	mms-ontology:key "isDerived" ;
	rdfs:label "isDerivedProperty" ;
	rdfs:comment "Specifies whether the Property is derived, i.e., whether its value or values can be computed from other information."@en ;
	rdfs:domain uml-class:Property ;
	rdfs:range xsd:boolean ;
	mms-ontology:umlPropertySource uml-property:Property-isDerived .

mms-property:isDerivedAssociation a mms-ontology:UmlDatatypeProperty ;
	mms-ontology:key "isDerived" ;
	rdfs:label "isDerivedAssociation" ;
	rdfs:comment "Specifies whether the Association is derived from other model elements such as other Associations."@en ;
	rdfs:domain uml-class:Association ;
	rdfs:range xsd:boolean ;
	mms-ontology:umlPropertySource uml-property:Association-isDerived .

mms-property:isDerivedUnion a mms-ontology:UmlDatatypeProperty ;
	mms-ontology:key "isDerivedUnion" ;
	rdfs:label "isDerivedUnion" ;
	rdfs:comment "Specifies whether the property is derived as the union of all of the Properties that are constrained to subset it."@en ;
	rdfs:domain uml-class:Property ;
	rdfs:range xsd:boolean ;
	mms-ontology:umlPropertySource uml-property:Property-isDerivedUnion .

mms-property:isDerivedUnionProperty a mms-ontology:UmlDatatypeProperty ;
	owl:equivalentProperty mms-property:isDerivedUnion .

mms-property:isDimension a mms-ontology:UmlDatatypeProperty ;
	mms-ontology:key "isDimension" ;
	rdfs:label "isDimension" ;
	rdfs:comment "Indicates whether the ActivityPartition groups other ActivityPartitions along a dimension."@en ;
	rdfs:domain uml-class:ActivityPartition ;
	rdfs:range xsd:boolean ;
	mms-ontology:umlPropertySource uml-property:ActivityPartition-isDimension .

mms-property:isDimensionActivityPartition a mms-ontology:UmlDatatypeProperty ;
	owl:equivalentProperty mms-property:isDimension .

mms-property:isException a mms-ontology:UmlDatatypeProperty ;
	mms-ontology:key "isException" ;
	rdfs:label "isException" ;
	rdfs:comment "Tells whether an output parameter may emit a value to the exclusion of the other outputs."@en ;
	rdfs:domain uml-class:Parameter ;
	rdfs:range xsd:boolean ;
	mms-ontology:umlPropertySource uml-property:Parameter-isException .

mms-property:isExceptionParameter a mms-ontology:UmlDatatypeProperty ;
	owl:equivalentProperty mms-property:isException .

mms-property:isExternal a mms-ontology:UmlDatatypeProperty ;
	mms-ontology:key "isExternal" ;
	rdfs:label "isExternal" ;
	rdfs:comment "Indicates whether the ActivityPartition represents an entity to which the partitioning structure does not apply."@en ;
	rdfs:domain uml-class:ActivityPartition ;
	rdfs:range xsd:boolean ;
	mms-ontology:umlPropertySource uml-property:ActivityPartition-isExternal .

mms-property:isExternalActivityPartition a mms-ontology:UmlDatatypeProperty ;
	owl:equivalentProperty mms-property:isExternal .

mms-property:isFinalSpecialization a mms-ontology:UmlDatatypeProperty ;
	mms-ontology:key "isFinalSpecialization" ;
	rdfs:label "isFinalSpecialization" ;
	rdfs:comment "If true, the Classifier cannot be specialized."@en ;
	rdfs:domain uml-class:Classifier ;
	rdfs:range xsd:boolean ;
	mms-ontology:umlPropertySource uml-property:Classifier-isFinalSpecialization .

mms-property:isFinalSpecializationClassifier a mms-ontology:UmlDatatypeProperty ;
	owl:equivalentProperty mms-property:isFinalSpecialization .

mms-property:isID a mms-ontology:UmlDatatypeProperty ;
	mms-ontology:key "isID" ;
	rdfs:label "isID" ;
	rdfs:comment "True indicates this property can be used to uniquely identify an instance of the containing Class."@en ;
	rdfs:domain uml-class:Property ;
	rdfs:range xsd:boolean ;
	mms-ontology:umlPropertySource uml-property:Property-isID .

mms-property:isIDProperty a mms-ontology:UmlDatatypeProperty ;
	owl:equivalentProperty mms-property:isID .

mms-property:isIndirectlyInstantiated a mms-ontology:UmlDatatypeProperty ;
	mms-ontology:key "isIndirectlyInstantiated" ;
	rdfs:label "isIndirectlyInstantiated" ;
	rdfs:comment "If true, the Component is defined at design-time, but at run-time (or execution-time) an object specified by the Component does not exist, that is, the Component is instantiated indirectly, through the instantiation of its realizing Classifiers or parts."@en ;
	rdfs:domain uml-class:Component ;
	rdfs:range xsd:boolean ;
	mms-ontology:umlPropertySource uml-property:Component-isIndirectlyInstantiated .

mms-property:isIndirectlyInstantiatedComponent a mms-ontology:UmlDatatypeProperty ;
	owl:equivalentProperty mms-property:isIndirectlyInstantiated .

mms-property:isLeaf a mms-ontology:UmlDatatypeProperty ;
	mms-ontology:key "isLeaf" ;
	rdfs:label "isLeaf" ;
	rdfs:comment "Indicates whether it is possible to further redefine a RedefinableElement. If the value is true, then it is not possible to further redefine the RedefinableElement."@en ;
	rdfs:domain uml-class:RedefinableElement ;
	rdfs:range xsd:boolean ;
	mms-ontology:umlPropertySource uml-property:RedefinableElement-isLeaf .

mms-property:isLeafRedefinableElement a mms-ontology:UmlDatatypeProperty ;
	owl:equivalentProperty mms-property:isLeaf .

mms-property:isLocallyReentrant a mms-ontology:UmlDatatypeProperty ;
	mms-ontology:key "isLocallyReentrant" ;
	rdfs:label "isLocallyReentrant" ;
	rdfs:comment "If true, the Action can begin a new, concurrent execution, even if there is already another execution of the Action ongoing. If false, the Action cannot begin a new execution until any previous execution has completed."@en ;
	rdfs:domain uml-class:Action ;
	rdfs:range xsd:boolean ;
	mms-ontology:umlPropertySource uml-property:Action-isLocallyReentrant .

mms-property:isLocallyReentrantAction a mms-ontology:UmlDatatypeProperty ;
	owl:equivalentProperty mms-property:isLocallyReentrant .

mms-property:isMulticast a mms-ontology:UmlDatatypeProperty ;
	mms-ontology:key "isMulticast" ;
	rdfs:label "isMulticast" ;
	rdfs:comment "Indicates whether the objects in the ObjectFlow are passed by multicasting."@en ;
	rdfs:domain uml-class:ObjectFlow ;
	rdfs:range xsd:boolean ;
	mms-ontology:umlPropertySource uml-property:ObjectFlow-isMulticast .

mms-property:isMulticastObjectFlow a mms-ontology:UmlDatatypeProperty ;
	owl:equivalentProperty mms-property:isMulticast .

mms-property:isMultireceive a mms-ontology:UmlDatatypeProperty ;
	mms-ontology:key "isMultireceive" ;
	rdfs:label "isMultireceive" ;
	rdfs:comment "Indicates whether the objects in the ObjectFlow are gathered from respondents to multicasting."@en ;
	rdfs:domain uml-class:ObjectFlow ;
	rdfs:range xsd:boolean ;
	mms-ontology:umlPropertySource uml-property:ObjectFlow-isMultireceive .

mms-property:isMultireceiveObjectFlow a mms-ontology:UmlDatatypeProperty ;
	owl:equivalentProperty mms-property:isMultireceive .

mms-property:isOrderedOperation a mms-ontology:UmlDatatypeProperty ;
	mms-ontology:key "isOrdered" ;
	rdfs:label "isOrderedOperation" ;
	rdfs:comment "Specifies whether the return parameter is ordered or not, if present.  This information is derived from the return result for this Operation."@en ;
	rdfs:domain uml-class:Operation ;
	rdfs:range xsd:boolean ;
	mms-ontology:umlPropertySource uml-property:Operation-isOrdered .

mms-property:isOrderedReduceAction a mms-ontology:UmlDatatypeProperty ;
	mms-ontology:key "isOrdered" ;
	rdfs:label "isOrderedReduceAction" ;
	rdfs:comment "Indicates whether the order of the input collection should determine the order in which the reducer Behavior is applied to its elements."@en ;
	rdfs:domain uml-class:ReduceAction ;
	rdfs:range xsd:boolean ;
	mms-ontology:umlPropertySource uml-property:ReduceAction-isOrdered .

mms-property:isOrderedMultiplicityElement a mms-ontology:UmlDatatypeProperty ;
	mms-ontology:key "isOrdered" ;
	rdfs:label "isOrderedMultiplicityElement" ;
	rdfs:comment "For a multivalued multiplicity, this attribute specifies whether the values in an instantiation of this MultiplicityElement are sequentially ordered."@en ;
	rdfs:domain uml-class:MultiplicityElement ;
	rdfs:range xsd:boolean ;
	mms-ontology:umlPropertySource uml-property:MultiplicityElement-isOrdered .

mms-property:isQuery a mms-ontology:UmlDatatypeProperty ;
	mms-ontology:key "isQuery" ;
	rdfs:label "isQuery" ;
	rdfs:comment "Specifies whether an execution of the BehavioralFeature leaves the state of the system unchanged (isQuery=true) or whether side effects may occur (isQuery=false)."@en ;
	rdfs:domain uml-class:Operation ;
	rdfs:range xsd:boolean ;
	mms-ontology:umlPropertySource uml-property:Operation-isQuery .

mms-property:isQueryOperation a mms-ontology:UmlDatatypeProperty ;
	owl:equivalentProperty mms-property:isQuery .

mms-property:isReadOnlyStructuralFeature a mms-ontology:UmlDatatypeProperty ;
	mms-ontology:key "isReadOnly" ;
	rdfs:label "isReadOnlyStructuralFeature" ;
	rdfs:comment "If isReadOnly is true, the StructuralFeature may not be written to after initialization."@en ;
	rdfs:domain uml-class:StructuralFeature ;
	rdfs:range xsd:boolean ;
	mms-ontology:umlPropertySource uml-property:StructuralFeature-isReadOnly .

mms-property:isReadOnlyActivity a mms-ontology:UmlDatatypeProperty ;
	mms-ontology:key "isReadOnly" ;
	rdfs:label "isReadOnlyActivity" ;
	rdfs:comment "If true, this Activity must not make any changes to objects. The default is false (an Activity may make nonlocal changes). (This is an assertion, not an executable property. It may be used by an execution engine to optimize model execution. If the assertion is violated by the Activity, then the model is ill-formed.) "@en ;
	rdfs:domain uml-class:Activity ;
	rdfs:range xsd:boolean ;
	mms-ontology:umlPropertySource uml-property:Activity-isReadOnly .

mms-property:isReentrant a mms-ontology:UmlDatatypeProperty ;
	mms-ontology:key "isReentrant" ;
	rdfs:label "isReentrant" ;
	rdfs:comment "Tells whether the Behavior can be invoked while it is still executing from a previous invocation."@en ;
	rdfs:domain uml-class:Behavior ;
	rdfs:range xsd:boolean ;
	mms-ontology:umlPropertySource uml-property:Behavior-isReentrant .

mms-property:isReentrantBehavior a mms-ontology:UmlDatatypeProperty ;
	owl:equivalentProperty mms-property:isReentrant .

mms-property:isRelative a mms-ontology:UmlDatatypeProperty ;
	mms-ontology:key "isRelative" ;
	rdfs:label "isRelative" ;
	rdfs:comment "Specifies whether the TimeEvent is specified as an absolute or relative time."@en ;
	rdfs:domain uml-class:TimeEvent ;
	rdfs:range xsd:boolean ;
	mms-ontology:umlPropertySource uml-property:TimeEvent-isRelative .

mms-property:isRelativeTimeEvent a mms-ontology:UmlDatatypeProperty ;
	owl:equivalentProperty mms-property:isRelative .

mms-property:isReplaceAllReclassifyObjectAction a mms-ontology:UmlDatatypeProperty ;
	mms-ontology:key "isReplaceAll" ;
	rdfs:label "isReplaceAllReclassifyObjectAction" ;
	rdfs:comment "Specifies whether existing Classifiers should be removed before adding the new Classifiers."@en ;
	rdfs:domain uml-class:ReclassifyObjectAction ;
	rdfs:range xsd:boolean ;
	mms-ontology:umlPropertySource uml-property:ReclassifyObjectAction-isReplaceAll .

mms-property:isReplaceAllAddVariableValueAction a mms-ontology:UmlDatatypeProperty ;
	mms-ontology:key "isReplaceAll" ;
	rdfs:label "isReplaceAllAddVariableValueAction" ;
	rdfs:comment "Specifies whether existing values of the Variable should be removed before adding the new value."@en ;
	rdfs:domain uml-class:AddVariableValueAction ;
	rdfs:range xsd:boolean ;
	mms-ontology:umlPropertySource uml-property:AddVariableValueAction-isReplaceAll .

mms-property:isReplaceAllAddStructuralFeatureValueAction a mms-ontology:UmlDatatypeProperty ;
	mms-ontology:key "isReplaceAll" ;
	rdfs:label "isReplaceAllAddStructuralFeatureValueAction" ;
	rdfs:comment "Specifies whether existing values of the StructuralFeature should be removed before adding the new value."@en ;
	rdfs:domain uml-class:AddStructuralFeatureValueAction ;
	rdfs:range xsd:boolean ;
	mms-ontology:umlPropertySource uml-property:AddStructuralFeatureValueAction-isReplaceAll .

mms-property:isReplaceAllLinkEndCreationData a mms-ontology:UmlDatatypeProperty ;
	mms-ontology:key "isReplaceAll" ;
	rdfs:label "isReplaceAllLinkEndCreationData" ;
	rdfs:comment "Specifies whether the existing links emanating from the object on this end should be destroyed before creating a new link."@en ;
	rdfs:domain uml-class:LinkEndCreationData ;
	rdfs:range xsd:boolean ;
	mms-ontology:umlPropertySource uml-property:LinkEndCreationData-isReplaceAll .

mms-property:isService a mms-ontology:UmlDatatypeProperty ;
	mms-ontology:key "isService" ;
	rdfs:label "isService" ;
	rdfs:comment "If true, indicates that this Port is used to provide the published functionality of an EncapsulatedClassifier.  If false, this Port is used to implement the EncapsulatedClassifier but is not part of the essential externally-visible functionality of the EncapsulatedClassifier and can, therefore, be altered or deleted along with the internal implementation of the EncapsulatedClassifier and other properties that are considered part of its implementation."@en ;
	rdfs:domain uml-class:Port ;
	rdfs:range xsd:boolean ;
	mms-ontology:umlPropertySource uml-property:Port-isService .

mms-property:isServicePort a mms-ontology:UmlDatatypeProperty ;
	owl:equivalentProperty mms-property:isService .

mms-property:isSingleExecution a mms-ontology:UmlDatatypeProperty ;
	mms-ontology:key "isSingleExecution" ;
	rdfs:label "isSingleExecution" ;
	rdfs:comment "If true, all invocations of the Activity are handled by the same execution."@en ;
	rdfs:domain uml-class:Activity ;
	rdfs:range xsd:boolean ;
	mms-ontology:umlPropertySource uml-property:Activity-isSingleExecution .

mms-property:isSingleExecutionActivity a mms-ontology:UmlDatatypeProperty ;
	owl:equivalentProperty mms-property:isSingleExecution .

mms-property:isStatic a mms-ontology:UmlDatatypeProperty ;
	mms-ontology:key "isStatic" ;
	rdfs:label "isStatic" ;
	rdfs:comment "Specifies whether this Feature characterizes individual instances classified by the Classifier (false) or the Classifier itself (true)."@en ;
	rdfs:domain uml-class:Feature ;
	rdfs:range xsd:boolean ;
	mms-ontology:umlPropertySource uml-property:Feature-isStatic .

mms-property:isStaticFeature a mms-ontology:UmlDatatypeProperty ;
	owl:equivalentProperty mms-property:isStatic .

mms-property:isStream a mms-ontology:UmlDatatypeProperty ;
	mms-ontology:key "isStream" ;
	rdfs:label "isStream" ;
	rdfs:comment "Tells whether an input parameter may accept values while its behavior is executing, or whether an output parameter may post values while the behavior is executing."@en ;
	rdfs:domain uml-class:Parameter ;
	rdfs:range xsd:boolean ;
	mms-ontology:umlPropertySource uml-property:Parameter-isStream .

mms-property:isStreamParameter a mms-ontology:UmlDatatypeProperty ;
	owl:equivalentProperty mms-property:isStream .

mms-property:isStrict a mms-ontology:UmlDatatypeProperty ;
	mms-ontology:key "isStrict" ;
	rdfs:label "isStrict" ;
	rdfs:comment "Specifies that the Profile filtering rules for the metaclasses of the referenced metamodel shall be strictly applied."@en ;
	rdfs:domain uml-class:ProfileApplication ;
	rdfs:range xsd:boolean ;
	mms-ontology:umlPropertySource uml-property:ProfileApplication-isStrict .

mms-property:isStrictProfileApplication a mms-ontology:UmlDatatypeProperty ;
	owl:equivalentProperty mms-property:isStrict .

mms-property:isSubstitutable a mms-ontology:UmlDatatypeProperty ;
	mms-ontology:key "isSubstitutable" ;
	rdfs:label "isSubstitutable" ;
	rdfs:comment "Indicates whether the specific Classifier can be used wherever the general Classifier can be used. If true, the execution traces of the specific Classifier shall be a superset of the execution traces of the general Classifier. If false, there is no such constraint on execution traces. If unset, the modeler has not stated whether there is such a constraint or not."@en ;
	rdfs:domain uml-class:Generalization ;
	rdfs:range xsd:boolean ;
	mms-ontology:umlPropertySource uml-property:Generalization-isSubstitutable .

mms-property:isSubstitutableGeneralization a mms-ontology:UmlDatatypeProperty ;
	owl:equivalentProperty mms-property:isSubstitutable .

mms-property:isSynchronous a mms-ontology:UmlDatatypeProperty ;
	mms-ontology:key "isSynchronous" ;
	rdfs:label "isSynchronous" ;
	rdfs:comment "If true, the call is synchronous and the caller waits for completion of the invoked Behavior. If false, the call is asynchronous and the caller proceeds immediately and cannot receive return values."@en ;
	rdfs:domain uml-class:CallAction ;
	rdfs:range xsd:boolean ;
	mms-ontology:umlPropertySource uml-property:CallAction-isSynchronous .

mms-property:isSynchronousCallAction a mms-ontology:UmlDatatypeProperty ;
	owl:equivalentProperty mms-property:isSynchronous .

mms-property:isTestedFirst a mms-ontology:UmlDatatypeProperty ;
	mms-ontology:key "isTestedFirst" ;
	rdfs:label "isTestedFirst" ;
	rdfs:comment "If true, the test is performed before the first execution of the bodyPart. If false, the bodyPart is executed once before the test is performed."@en ;
	rdfs:domain uml-class:LoopNode ;
	rdfs:range xsd:boolean ;
	mms-ontology:umlPropertySource uml-property:LoopNode-isTestedFirst .

mms-property:isTestedFirstLoopNode a mms-ontology:UmlDatatypeProperty ;
	owl:equivalentProperty mms-property:isTestedFirst .

mms-property:isUniqueOperation a mms-ontology:UmlDatatypeProperty ;
	mms-ontology:key "isUnique" ;
	rdfs:label "isUniqueOperation" ;
	rdfs:comment "Specifies whether the return parameter is unique or not, if present. This information is derived from the return result for this Operation."@en ;
	rdfs:domain uml-class:Operation ;
	rdfs:range xsd:boolean ;
	mms-ontology:umlPropertySource uml-property:Operation-isUnique .

mms-property:isUniqueMultiplicityElement a mms-ontology:UmlDatatypeProperty ;
	mms-ontology:key "isUnique" ;
	rdfs:label "isUniqueMultiplicityElement" ;
	rdfs:comment "For a multivalued multiplicity, this attributes specifies whether the values in an instantiation of this MultiplicityElement are unique."@en ;
	rdfs:domain uml-class:MultiplicityElement ;
	rdfs:range xsd:boolean ;
	mms-ontology:umlPropertySource uml-property:MultiplicityElement-isUnique .

mms-property:isUnmarshall a mms-ontology:UmlDatatypeProperty ;
	mms-ontology:key "isUnmarshall" ;
	rdfs:label "isUnmarshall" ;
	rdfs:comment "Indicates whether there is a single OutputPin for a SignalEvent occurrence, or multiple OutputPins for attribute values of the instance of the Signal associated with a SignalEvent occurrence."@en ;
	rdfs:domain uml-class:AcceptEventAction ;
	rdfs:range xsd:boolean ;
	mms-ontology:umlPropertySource uml-property:AcceptEventAction-isUnmarshall .

mms-property:isUnmarshallAcceptEventAction a mms-ontology:UmlDatatypeProperty ;
	owl:equivalentProperty mms-property:isUnmarshall .

mms-property:lifeline a mms-ontology:UmlObjectProperty ;
	mms-ontology:key "lifelineIds" ;
	rdfs:label "lifeline" ;
	rdfs:comment "A Lifeline that belongs to this Interaction. Based on the UML property 'Interaction-lifeline' which is described as: Specifies the participants in this Interaction.."@en ;
	rdfs:domain uml-class:Interaction ;
	rdfs:range uml-class:Lifeline ;
	mms-ontology:umlPropertySource uml-property:Interaction-lifeline .

mms-property:memberEnd a mms-ontology:UmlObjectProperty ;
	mms-ontology:key "memberEndIds" ;
	rdfs:label "memberEnd" ;
	rdfs:comment "A Property that is the memberEnd of this Association. Based on the UML property 'Association-memberEnd' which is described as: Each end represents participation of instances of the Classifier connected to the end in links of the Association.."@en ;
	rdfs:domain uml-class:Association ;
	rdfs:range uml-class:Property ;
	mms-ontology:umlPropertySource uml-property:Association-memberEnd .

mms-property:messageFromMessageEnd a mms-ontology:UmlObjectProperty ;
	mms-ontology:key "messageId" ;
	rdfs:label "messageFromMessageEnd" ;
	rdfs:comment "The Message that belongs to this MessageEnd. Based on the UML property 'MessageEnd-message' which is described as: References a Message.."@en ;
	rdfs:domain uml-class:MessageEnd ;
	rdfs:range uml-class:Message ;
	mms-ontology:umlPropertySource uml-property:MessageEnd-message .

mms-property:messageFromInteraction a mms-ontology:UmlObjectProperty ;
	mms-ontology:key "messageId" ;
	rdfs:label "messageFromInteraction" ;
	rdfs:comment "The Message that belongs to this Interaction. Based on the UML property 'Interaction-message' which is described as: The Messages contained in this Interaction.."@en ;
	rdfs:domain uml-class:Interaction ;
	rdfs:range uml-class:Message ;
	mms-ontology:umlPropertySource uml-property:Interaction-message .

mms-property:messageNamedElement a mms-ontology:UmlObjectProperty ;
	mms-ontology:key "messageId" ;
	rdfs:label "messageNamedElement" ;
	rdfs:comment "The NamedElement that is the message of this ConsiderIgnoreFragment. Based on the UML property 'ConsiderIgnoreFragment-message' which is described as: The set of messages that apply to this fragment.."@en ;
	rdfs:domain uml-class:ConsiderIgnoreFragment ;
	rdfs:range uml-class:NamedElement ;
	mms-ontology:umlPropertySource uml-property:ConsiderIgnoreFragment-message .

mms-property:messageFromMessageEnd a mms-ontology:UmlObjectProperty ;
	mms-ontology:key "messageIds" ;
	rdfs:label "messageFromMessageEnd" ;
	rdfs:comment "The Message that belongs to this MessageEnd. Based on the UML property 'MessageEnd-message' which is described as: References a Message.."@en ;
	rdfs:domain uml-class:MessageEnd ;
	rdfs:range uml-class:Message ;
	mms-ontology:umlPropertySource uml-property:MessageEnd-message .

mms-property:messageFromInteraction a mms-ontology:UmlObjectProperty ;
	mms-ontology:key "messageIds" ;
	rdfs:label "messageFromInteraction" ;
	rdfs:comment "A Message that belongs to this Interaction. Based on the UML property 'Interaction-message' which is described as: The Messages contained in this Interaction.."@en ;
	rdfs:domain uml-class:Interaction ;
	rdfs:range uml-class:Message ;
	mms-ontology:umlPropertySource uml-property:Interaction-message .

mms-property:messageNamedElement a mms-ontology:UmlObjectProperty ;
	mms-ontology:key "messageIds" ;
	rdfs:label "messageNamedElement" ;
	rdfs:comment "A NamedElement that is the message of this ConsiderIgnoreFragment. Based on the UML property 'ConsiderIgnoreFragment-message' which is described as: The set of messages that apply to this fragment.."@en ;
	rdfs:domain uml-class:ConsiderIgnoreFragment ;
	rdfs:range uml-class:NamedElement ;
	mms-ontology:umlPropertySource uml-property:ConsiderIgnoreFragment-message .

mms-property:metamodelReference a mms-ontology:UmlObjectProperty ;
	mms-ontology:key "metamodelReferenceIds" ;
	rdfs:label "metamodelReference" ;
	rdfs:comment "A PackageImport that is the metamodelReference of this Profile. Based on the UML property 'Profile-metamodelReference' which is described as: References a package containing (directly or indirectly) metaclasses that may be extended.."@en ;
	rdfs:domain uml-class:Profile ;
	rdfs:range uml-class:PackageImport ;
	mms-ontology:umlPropertySource uml-property:Profile-metamodelReference .

mms-property:method a mms-ontology:UmlObjectProperty ;
	mms-ontology:key "methodIds" ;
	rdfs:label "method" ;
	rdfs:comment "A Behavior that is the method of this BehavioralFeature. Based on the UML property 'BehavioralFeature-method' which is described as: A Behavior that implements the BehavioralFeature. There may be at most one Behavior for a particular pairing of a Classifier (as owner of the Behavior) and a BehavioralFeature (as specification of the Behavior).."@en ;
	rdfs:domain uml-class:BehavioralFeature ;
	rdfs:range uml-class:Behavior ;
	mms-ontology:umlPropertySource uml-property:BehavioralFeature-method .

mms-property:navigableOwnedEnd a mms-ontology:UmlObjectProperty ;
	mms-ontology:key "navigableOwnedEndIds" ;
	rdfs:label "navigableOwnedEnd" ;
	rdfs:comment "A Property that is the navigableOwnedEnd of this Association. Based on the UML property 'Association-navigableOwnedEnd' which is described as: The navigable ends that are owned by the Association itself.."@en ;
	rdfs:domain uml-class:Association ;
	rdfs:range uml-class:Property ;
	mms-ontology:umlPropertySource uml-property:Association-navigableOwnedEnd .

mms-property:nodeFromActivityPartition a mms-ontology:UmlObjectProperty ;
	mms-ontology:key "nodeIds" ;
	rdfs:label "nodeFromActivityPartition" ;
	rdfs:comment "A ActivityNode that is the node of this ActivityPartition. Based on the UML property 'ActivityPartition-node' which is described as: ActivityNodes immediately contained in the ActivityPartition.."@en ;
	rdfs:domain uml-class:ActivityPartition ;
	rdfs:range uml-class:ActivityNode ;
	mms-ontology:umlPropertySource uml-property:ActivityPartition-node .

mms-property:nodeFromInterruptibleActivityRegion a mms-ontology:UmlObjectProperty ;
	mms-ontology:key "nodeIds" ;
	rdfs:label "nodeFromInterruptibleActivityRegion" ;
	rdfs:comment "A ActivityNode that is the node of this InterruptibleActivityRegion. Based on the UML property 'InterruptibleActivityRegion-node' which is described as: ActivityNodes immediately contained in the InterruptibleActivityRegion.."@en ;
	rdfs:domain uml-class:InterruptibleActivityRegion ;
	rdfs:range uml-class:ActivityNode ;
	mms-ontology:umlPropertySource uml-property:InterruptibleActivityRegion-node .

mms-property:nodeFromStructuredActivityNode a mms-ontology:UmlObjectProperty ;
	mms-ontology:key "nodeIds" ;
	rdfs:label "nodeFromStructuredActivityNode" ;
	rdfs:comment "A ActivityNode that is the node of this StructuredActivityNode. Based on the UML property 'StructuredActivityNode-node' which is described as: The ActivityNodes immediately contained in the StructuredActivityNode.."@en ;
	rdfs:domain uml-class:StructuredActivityNode ;
	rdfs:range uml-class:ActivityNode ;
	mms-ontology:umlPropertySource uml-property:StructuredActivityNode-node .

mms-property:nodeFromActivity a mms-ontology:UmlObjectProperty ;
	mms-ontology:key "nodeIds" ;
	rdfs:label "nodeFromActivity" ;
	rdfs:comment "A ActivityNode that is the node of this Activity. Based on the UML property 'Activity-node' which is described as: ActivityNodes coordinated by the Activity.."@en ;
	rdfs:domain uml-class:Activity ;
	rdfs:range uml-class:ActivityNode ;
	mms-ontology:umlPropertySource uml-property:Activity-node .

mms-property:objectInputPinFromStructuralFeatureAction a mms-ontology:UmlObjectProperty ;
	mms-ontology:key "objectId" ;
	rdfs:label "objectInputPinFromStructuralFeatureAction" ;
	rdfs:comment "The InputPin that is the object of this StructuralFeatureAction. Based on the UML property 'StructuralFeatureAction-object' which is described as: The InputPin from which the object whose StructuralFeature is to be read or written is obtained.."@en ;
	rdfs:domain uml-class:StructuralFeatureAction ;
	rdfs:range uml-class:InputPin ;
	mms-ontology:umlPropertySource uml-property:StructuralFeatureAction-object .

mms-property:objectInputPinFromReadLinkObjectEndAction a mms-ontology:UmlObjectProperty ;
	mms-ontology:key "objectId" ;
	rdfs:label "objectInputPinFromReadLinkObjectEndAction" ;
	rdfs:comment "The InputPin that is the object of this ReadLinkObjectEndAction. Based on the UML property 'ReadLinkObjectEndAction-object' which is described as: The input pin from which the link object is obtained.."@en ;
	rdfs:domain uml-class:ReadLinkObjectEndAction ;
	rdfs:range uml-class:InputPin ;
	mms-ontology:umlPropertySource uml-property:ReadLinkObjectEndAction-object .

mms-property:objectInputPinFromClearAssociationAction a mms-ontology:UmlObjectProperty ;
	mms-ontology:key "objectId" ;
	rdfs:label "objectInputPinFromClearAssociationAction" ;
	rdfs:comment "The InputPin that is the object of this ClearAssociationAction. Based on the UML property 'ClearAssociationAction-object' which is described as: The InputPin that gives the object whose participation in the Association is to be cleared.."@en ;
	rdfs:domain uml-class:ClearAssociationAction ;
	rdfs:range uml-class:InputPin ;
	mms-ontology:umlPropertySource uml-property:ClearAssociationAction-object .

mms-property:objectInputPinFromStartObjectBehaviorAction a mms-ontology:UmlObjectProperty ;
	mms-ontology:key "objectId" ;
	rdfs:label "objectInputPinFromStartObjectBehaviorAction" ;
	rdfs:comment "The InputPin that is the object of this StartObjectBehaviorAction. Based on the UML property 'StartObjectBehaviorAction-object' which is described as: An InputPin that holds the object that is either a Behavior to be started or has a classifierBehavior to be started.."@en ;
	rdfs:domain uml-class:StartObjectBehaviorAction ;
	rdfs:range uml-class:InputPin ;
	mms-ontology:umlPropertySource uml-property:StartObjectBehaviorAction-object .

mms-property:objectInputPinFromReadIsClassifiedObjectAction a mms-ontology:UmlObjectProperty ;
	mms-ontology:key "objectId" ;
	rdfs:label "objectInputPinFromReadIsClassifiedObjectAction" ;
	rdfs:comment "The InputPin that is the object of this ReadIsClassifiedObjectAction. Based on the UML property 'ReadIsClassifiedObjectAction-object' which is described as: The InputPin that holds the object whose classification is to be tested.."@en ;
	rdfs:domain uml-class:ReadIsClassifiedObjectAction ;
	rdfs:range uml-class:InputPin ;
	mms-ontology:umlPropertySource uml-property:ReadIsClassifiedObjectAction-object .

mms-property:objectInputPinFromReclassifyObjectAction a mms-ontology:UmlObjectProperty ;
	mms-ontology:key "objectId" ;
	rdfs:label "objectInputPinFromReclassifyObjectAction" ;
	rdfs:comment "The InputPin that is the object of this ReclassifyObjectAction. Based on the UML property 'ReclassifyObjectAction-object' which is described as: The InputPin that holds the object to be reclassified.."@en ;
	rdfs:domain uml-class:ReclassifyObjectAction ;
	rdfs:range uml-class:InputPin ;
	mms-ontology:umlPropertySource uml-property:ReclassifyObjectAction-object .

mms-property:objectInputPinFromStartClassifierBehaviorAction a mms-ontology:UmlObjectProperty ;
	mms-ontology:key "objectId" ;
	rdfs:label "objectInputPinFromStartClassifierBehaviorAction" ;
	rdfs:comment "The InputPin that is the object of this StartClassifierBehaviorAction. Based on the UML property 'StartClassifierBehaviorAction-object' which is described as: The InputPin that holds the object whose classifierBehavior is to be started.."@en ;
	rdfs:domain uml-class:StartClassifierBehaviorAction ;
	rdfs:range uml-class:InputPin ;
	mms-ontology:umlPropertySource uml-property:StartClassifierBehaviorAction-object .

mms-property:objectInputPinFromReadLinkObjectEndQualifierAction a mms-ontology:UmlObjectProperty ;
	mms-ontology:key "objectId" ;
	rdfs:label "objectInputPinFromReadLinkObjectEndQualifierAction" ;
	rdfs:comment "The InputPin that is the object of this ReadLinkObjectEndQualifierAction. Based on the UML property 'ReadLinkObjectEndQualifierAction-object' which is described as: The InputPin from which the link object is obtained.."@en ;
	rdfs:domain uml-class:ReadLinkObjectEndQualifierAction ;
	rdfs:range uml-class:InputPin ;
	mms-ontology:umlPropertySource uml-property:ReadLinkObjectEndQualifierAction-object .

mms-property:objectInputPinFromUnmarshallAction a mms-ontology:UmlObjectProperty ;
	mms-ontology:key "objectId" ;
	rdfs:label "objectInputPinFromUnmarshallAction" ;
	rdfs:comment "The InputPin that is the object of this UnmarshallAction. Based on the UML property 'UnmarshallAction-object' which is described as: The InputPin that gives the object to be unmarshalled.."@en ;
	rdfs:domain uml-class:UnmarshallAction ;
	rdfs:range uml-class:InputPin ;
	mms-ontology:umlPropertySource uml-property:UnmarshallAction-object .

mms-property:observationFromTimeExpression a mms-ontology:UmlObjectProperty ;
	mms-ontology:key "observationIds" ;
	rdfs:label "observationFromTimeExpression" ;
	rdfs:comment "A Observation that belongs to this TimeExpression. Based on the UML property 'TimeExpression-observation' which is described as: Refers to the Observations that are involved in the computation of the TimeExpression value.."@en ;
	rdfs:domain uml-class:TimeExpression ;
	rdfs:range uml-class:Observation ;
	mms-ontology:umlPropertySource uml-property:TimeExpression-observation .

mms-property:observationFromDuration a mms-ontology:UmlObjectProperty ;
	mms-ontology:key "observationIds" ;
	rdfs:label "observationFromDuration" ;
	rdfs:comment "A Observation that belongs to this Duration. Based on the UML property 'Duration-observation' which is described as: Refers to the Observations that are involved in the computation of the Duration value."@en ;
	rdfs:domain uml-class:Duration ;
	rdfs:range uml-class:Observation ;
	mms-ontology:umlPropertySource uml-property:Duration-observation .

mms-property:onPort a mms-ontology:UmlObjectProperty ;
	mms-ontology:key "onPortId" ;
	rdfs:label "onPort" ;
	rdfs:comment "The Port that belongs to this InvocationAction. Based on the UML property 'InvocationAction-onPort' which is described as: For CallOperationActions, SendSignalActions, and SendObjectActions, an optional Port of the target object through which the invocation request is sent.."@en ;
	rdfs:domain uml-class:InvocationAction ;
	rdfs:range uml-class:Port ;
	mms-ontology:umlPropertySource uml-property:InvocationAction-onPort .

mms-property:operationFromCallEvent a mms-ontology:UmlObjectProperty ;
	mms-ontology:key "operationId" ;
	rdfs:label "operationFromCallEvent" ;
	rdfs:comment "The Operation that belongs to this CallEvent. Based on the UML property 'CallEvent-operation' which is described as: Designates the Operation whose invocation raised the CalEvent.."@en ;
	rdfs:domain uml-class:CallEvent ;
	rdfs:range uml-class:Operation ;
	mms-ontology:umlPropertySource uml-property:CallEvent-operation .

mms-property:operationFromCallOperationAction a mms-ontology:UmlObjectProperty ;
	mms-ontology:key "operationId" ;
	rdfs:label "operationFromCallOperationAction" ;
	rdfs:comment "The Operation that belongs to this CallOperationAction. Based on the UML property 'CallOperationAction-operation' which is described as: The Operation being invoked.."@en ;
	rdfs:domain uml-class:CallOperationAction ;
	rdfs:range uml-class:Operation ;
	mms-ontology:umlPropertySource uml-property:CallOperationAction-operation .

mms-property:operationFromParameter a mms-ontology:UmlObjectProperty ;
	mms-ontology:key "operationId" ;
	rdfs:label "operationFromParameter" ;
	rdfs:comment "The Operation that belongs to this Parameter. Based on the UML property 'Parameter-operation' which is described as: The Operation owning this parameter.."@en ;
	rdfs:domain uml-class:Parameter ;
	rdfs:range uml-class:Operation ;
	mms-ontology:umlPropertySource uml-property:Parameter-operation .

mms-property:outgoingActivityEdge a mms-ontology:UmlObjectProperty ;
	mms-ontology:key "outgoingIds" ;
	rdfs:label "outgoingActivityEdge" ;
	rdfs:comment "A ActivityEdge that is the outgoing of this ActivityNode. Based on the UML property 'ActivityNode-outgoing' which is described as: ActivityEdges that have the ActivityNode as their source.."@en ;
	rdfs:domain uml-class:ActivityNode ;
	rdfs:range uml-class:ActivityEdge ;
	mms-ontology:umlPropertySource uml-property:ActivityNode-outgoing .

mms-property:outgoingTransition a mms-ontology:UmlObjectProperty ;
	mms-ontology:key "outgoingIds" ;
	rdfs:label "outgoingTransition" ;
	rdfs:comment "A Transition that is the outgoing of this Vertex. Based on the UML property 'Vertex-outgoing' which is described as: Specifies the Transitions departing from this Vertex.."@en ;
	rdfs:domain uml-class:Vertex ;
	rdfs:range uml-class:Transition ;
	mms-ontology:umlPropertySource uml-property:Vertex-outgoing .

mms-property:outputValue a mms-ontology:UmlObjectProperty ;
	mms-ontology:key "outputValueIds" ;
	rdfs:label "outputValue" ;
	rdfs:comment "A OutputPin that is the outputValue of this OpaqueAction. Based on the UML property 'OpaqueAction-outputValue' which is described as: The OutputPins on which the OpaqueAction provides outputs.."@en ;
	rdfs:domain uml-class:OpaqueAction ;
	rdfs:range uml-class:OutputPin ;
	mms-ontology:umlPropertySource uml-property:OpaqueAction-outputValue .

mms-property:ownedAttributeFromSignal a mms-ontology:UmlObjectProperty ;
	mms-ontology:key "ownedAttributeIds" ;
	rdfs:label "ownedAttributeFromSignal" ;
	rdfs:comment "A Property that is the ownedAttribute of this Signal. Based on the UML property 'Signal-ownedAttribute' which is described as: The attributes owned by the Signal.."@en ;
	rdfs:domain uml-class:Signal ;
	rdfs:range uml-class:Property ;
	mms-ontology:umlPropertySource uml-property:Signal-ownedAttribute .

mms-property:ownedAttributeFromDataType a mms-ontology:UmlObjectProperty ;
	mms-ontology:key "ownedAttributeIds" ;
	rdfs:label "ownedAttributeFromDataType" ;
	rdfs:comment "A Property that is the ownedAttribute of this DataType. Based on the UML property 'DataType-ownedAttribute' which is described as: The attributes owned by the DataType.."@en ;
	rdfs:domain uml-class:DataType ;
	rdfs:range uml-class:Property ;
	mms-ontology:umlPropertySource uml-property:DataType-ownedAttribute .

mms-property:ownedAttributeFromArtifact a mms-ontology:UmlObjectProperty ;
	mms-ontology:key "ownedAttributeIds" ;
	rdfs:label "ownedAttributeFromArtifact" ;
	rdfs:comment "A Property that is the ownedAttribute of this Artifact. Based on the UML property 'Artifact-ownedAttribute' which is described as: The attributes or association ends defined for the Artifact. The association is a specialization of the ownedMember association.."@en ;
	rdfs:domain uml-class:Artifact ;
	rdfs:range uml-class:Property ;
	mms-ontology:umlPropertySource uml-property:Artifact-ownedAttribute .

mms-property:ownedAttributeFromClass a mms-ontology:UmlObjectProperty ;
	mms-ontology:key "ownedAttributeIds" ;
	rdfs:label "ownedAttributeFromClass" ;
	rdfs:comment "A Property that is the ownedAttribute of this Class. Based on the UML property 'Class-ownedAttribute' which is described as: The attributes (i.e., the Properties) owned by the Class.."@en ;
	rdfs:domain uml-class:Class ;
	rdfs:range uml-class:Property ;
	mms-ontology:umlPropertySource uml-property:Class-ownedAttribute .

mms-property:ownedAttributeFromStructuredClassifier a mms-ontology:UmlObjectProperty ;
	mms-ontology:key "ownedAttributeIds" ;
	rdfs:label "ownedAttributeFromStructuredClassifier" ;
	rdfs:comment "A Property that is the ownedAttribute of this StructuredClassifier. Based on the UML property 'StructuredClassifier-ownedAttribute' which is described as: The Properties owned by the StructuredClassifier.."@en ;
	rdfs:domain uml-class:StructuredClassifier ;
	rdfs:range uml-class:Property ;
	mms-ontology:umlPropertySource uml-property:StructuredClassifier-ownedAttribute .

mms-property:ownedAttributeFromInterface a mms-ontology:UmlObjectProperty ;
	mms-ontology:key "ownedAttributeIds" ;
	rdfs:label "ownedAttributeFromInterface" ;
	rdfs:comment "A Property that is the ownedAttribute of this Interface. Based on the UML property 'Interface-ownedAttribute' which is described as: The attributes (i.e., the Properties) owned by the Interface.."@en ;
	rdfs:domain uml-class:Interface ;
	rdfs:range uml-class:Property ;
	mms-ontology:umlPropertySource uml-property:Interface-ownedAttribute .

mms-property:ownedEndProperty a mms-ontology:UmlObjectProperty ;
	mms-ontology:key "ownedEndIds" ;
	rdfs:label "ownedEndProperty" ;
	rdfs:comment "A Property that is the ownedEnd of this Association. Based on the UML property 'Association-ownedEnd' which is described as: The ends that are owned by the Association itself.."@en ;
	rdfs:domain uml-class:Association ;
	rdfs:range uml-class:Property ;
	mms-ontology:umlPropertySource uml-property:Association-ownedEnd .

mms-property:ownedEndExtensionEnd a mms-ontology:UmlObjectProperty ;
	mms-ontology:key "ownedEndIds" ;
	rdfs:label "ownedEndExtensionEnd" ;
	rdfs:comment "The ExtensionEnd that is the ownedEnd of this Extension. Based on the UML property 'Extension-ownedEnd' which is described as: References the end of the extension that is typed by a Stereotype.."@en ;
	rdfs:domain uml-class:Extension ;
	rdfs:range uml-class:ExtensionEnd ;
	mms-ontology:umlPropertySource uml-property:Extension-ownedEnd .

mms-property:ownedLiteral a mms-ontology:UmlObjectProperty ;
	mms-ontology:key "ownedLiteralIds" ;
	rdfs:label "ownedLiteral" ;
	rdfs:comment "A EnumerationLiteral that is the ownedLiteral of this Enumeration. Based on the UML property 'Enumeration-ownedLiteral' which is described as: The ordered set of literals owned by this Enumeration.."@en ;
	rdfs:domain uml-class:Enumeration ;
	rdfs:range uml-class:EnumerationLiteral ;
	mms-ontology:umlPropertySource uml-property:Enumeration-ownedLiteral .

mms-property:ownedOperationFromInterface a mms-ontology:UmlObjectProperty ;
	mms-ontology:key "ownedOperationIds" ;
	rdfs:label "ownedOperationFromInterface" ;
	rdfs:comment "A Operation that belongs to this Interface. Based on the UML property 'Interface-ownedOperation' which is described as: The Operations owned by the Interface.."@en ;
	rdfs:domain uml-class:Interface ;
	rdfs:range uml-class:Operation ;
	mms-ontology:umlPropertySource uml-property:Interface-ownedOperation .

mms-property:ownedOperationFromClass a mms-ontology:UmlObjectProperty ;
	mms-ontology:key "ownedOperationIds" ;
	rdfs:label "ownedOperationFromClass" ;
	rdfs:comment "A Operation that belongs to this Class. Based on the UML property 'Class-ownedOperation' which is described as: The Operations owned by the Class.."@en ;
	rdfs:domain uml-class:Class ;
	rdfs:range uml-class:Operation ;
	mms-ontology:umlPropertySource uml-property:Class-ownedOperation .

mms-property:ownedOperationFromDataType a mms-ontology:UmlObjectProperty ;
	mms-ontology:key "ownedOperationIds" ;
	rdfs:label "ownedOperationFromDataType" ;
	rdfs:comment "A Operation that belongs to this DataType. Based on the UML property 'DataType-ownedOperation' which is described as: The Operations owned by the DataType.."@en ;
	rdfs:domain uml-class:DataType ;
	rdfs:range uml-class:Operation ;
	mms-ontology:umlPropertySource uml-property:DataType-ownedOperation .

mms-property:ownedOperationFromArtifact a mms-ontology:UmlObjectProperty ;
	mms-ontology:key "ownedOperationIds" ;
	rdfs:label "ownedOperationFromArtifact" ;
	rdfs:comment "A Operation that belongs to this Artifact. Based on the UML property 'Artifact-ownedOperation' which is described as: The Operations defined for the Artifact. The association is a specialization of the ownedMember association.."@en ;
	rdfs:domain uml-class:Artifact ;
	rdfs:range uml-class:Operation ;
	mms-ontology:umlPropertySource uml-property:Artifact-ownedOperation .

mms-property:ownedParameterTemplateParameter a mms-ontology:UmlObjectProperty ;
	mms-ontology:key "ownedParameterIds" ;
	rdfs:label "ownedParameterTemplateParameter" ;
	rdfs:comment "A TemplateParameter that is the ownedParameter of this TemplateSignature. Based on the UML property 'TemplateSignature-ownedParameter' which is described as: The formal parameters that are owned by this TemplateSignature.."@en ;
	rdfs:domain uml-class:TemplateSignature ;
	rdfs:range uml-class:TemplateParameter ;
	mms-ontology:umlPropertySource uml-property:TemplateSignature-ownedParameter .

mms-property:ownedParameterFromOperation a mms-ontology:UmlObjectProperty ;
	mms-ontology:key "ownedParameterIds" ;
	rdfs:label "ownedParameterFromOperation" ;
	rdfs:comment "A Parameter that belongs to this Operation. Based on the UML property 'Operation-ownedParameter' which is described as: The parameters owned by this Operation.."@en ;
	rdfs:domain uml-class:Operation ;
	rdfs:range uml-class:Parameter ;
	mms-ontology:umlPropertySource uml-property:Operation-ownedParameter .

mms-property:ownedParameterFromBehavior a mms-ontology:UmlObjectProperty ;
	mms-ontology:key "ownedParameterIds" ;
	rdfs:label "ownedParameterFromBehavior" ;
	rdfs:comment "A Parameter that belongs to this Behavior. Based on the UML property 'Behavior-ownedParameter' which is described as: References a list of Parameters to the Behavior which describes the order and type of arguments that can be given when the Behavior is invoked and of the values which will be returned when the Behavior completes its execution.."@en ;
	rdfs:domain uml-class:Behavior ;
	rdfs:range uml-class:Parameter ;
	mms-ontology:umlPropertySource uml-property:Behavior-ownedParameter .

mms-property:ownedParameterFromBehavioralFeature a mms-ontology:UmlObjectProperty ;
	mms-ontology:key "ownedParameterIds" ;
	rdfs:label "ownedParameterFromBehavioralFeature" ;
	rdfs:comment "A Parameter that belongs to this BehavioralFeature. Based on the UML property 'BehavioralFeature-ownedParameter' which is described as: The ordered set of formal Parameters of this BehavioralFeature.."@en ;
	rdfs:domain uml-class:BehavioralFeature ;
	rdfs:range uml-class:Parameter ;
	mms-ontology:umlPropertySource uml-property:BehavioralFeature-ownedParameter .

mms-property:ownerElement a mms-ontology:UmlObjectProperty ;
	mms-ontology:key "ownerId" ;
	rdfs:label "ownerElement" ;
	rdfs:comment "The Element that is the owner of this Element. Based on the UML property 'Element-owner' which is described as: The Element that owns this Element.."@en ;
	rdfs:domain uml-class:Element ;
	rdfs:range uml-class:Element ;
	mms-ontology:umlPropertySource uml-property:Element-owner .

mms-property:packageImport a mms-ontology:UmlObjectProperty ;
	mms-ontology:key "packageImportIds" ;
	rdfs:label "packageImport" ;
	rdfs:comment "A PackageImport that belongs to this Namespace. Based on the UML property 'Namespace-packageImport' which is described as: References the PackageImports owned by the Namespace.."@en ;
	rdfs:domain uml-class:Namespace ;
	rdfs:range uml-class:PackageImport ;
	mms-ontology:umlPropertySource uml-property:Namespace-packageImport .

mms-property:parameterTemplateParameter a mms-ontology:UmlObjectProperty ;
	mms-ontology:key "parameterId" ;
	rdfs:label "parameterTemplateParameter" ;
	rdfs:comment "The TemplateParameter that is the parameter of this TemplateSignature. Based on the UML property 'TemplateSignature-parameter' which is described as: The ordered set of all formal TemplateParameters for this TemplateSignature.."@en ;
	rdfs:domain uml-class:TemplateSignature ;
	rdfs:range uml-class:TemplateParameter ;
	mms-ontology:umlPropertySource uml-property:TemplateSignature-parameter .

mms-property:parameterFromParameterSet a mms-ontology:UmlObjectProperty ;
	mms-ontology:key "parameterId" ;
	rdfs:label "parameterFromParameterSet" ;
	rdfs:comment "The Parameter that belongs to this ParameterSet. Based on the UML property 'ParameterSet-parameter' which is described as: Parameters in the ParameterSet.."@en ;
	rdfs:domain uml-class:ParameterSet ;
	rdfs:range uml-class:Parameter ;
	mms-ontology:umlPropertySource uml-property:ParameterSet-parameter .

mms-property:parameterFromActivityParameterNode a mms-ontology:UmlObjectProperty ;
	mms-ontology:key "parameterId" ;
	rdfs:label "parameterFromActivityParameterNode" ;
	rdfs:comment "The Parameter that belongs to this ActivityParameterNode. Based on the UML property 'ActivityParameterNode-parameter' which is described as: The Parameter for which the ActivityParameterNode will be accepting or providing values.."@en ;
	rdfs:domain uml-class:ActivityParameterNode ;
	rdfs:range uml-class:Parameter ;
	mms-ontology:umlPropertySource uml-property:ActivityParameterNode-parameter .

mms-property:partWithPortProperty a mms-ontology:UmlObjectProperty ;
	mms-ontology:key "partWithPortId" ;
	rdfs:label "partWithPortProperty" ;
	rdfs:comment "The Property that is the partWithPort of this ConnectorEnd. Based on the UML property 'ConnectorEnd-partWithPort' which is described as: Indicates the role of the internal structure of a Classifier with the Port to which the ConnectorEnd is attached.."@en ;
	rdfs:domain uml-class:ConnectorEnd ;
	rdfs:range uml-class:Property ;
	mms-ontology:umlPropertySource uml-property:ConnectorEnd-partWithPort .

mms-property:partition a mms-ontology:UmlObjectProperty ;
	mms-ontology:key "partitionIds" ;
	rdfs:label "partition" ;
	rdfs:comment "A ActivityPartition that is the partition of this Activity. Based on the UML property 'Activity-partition' which is described as: Top-level ActivityPartitions in the Activity.."@en ;
	rdfs:domain uml-class:Activity ;
	rdfs:range uml-class:ActivityPartition ;
	mms-ontology:umlPropertySource uml-property:Activity-partition .

mms-property:port a mms-ontology:UmlObjectProperty ;
	mms-ontology:key "portIds" ;
	rdfs:label "port" ;
	rdfs:comment "A Port that belongs to this Trigger. Based on the UML property 'Trigger-port' which is described as: A optional Port of through which the given effect is detected.."@en ;
	rdfs:domain uml-class:Trigger ;
	rdfs:range uml-class:Port ;
	mms-ontology:umlPropertySource uml-property:Trigger-port .

mms-property:profileApplication a mms-ontology:UmlObjectProperty ;
	mms-ontology:key "profileApplicationIds" ;
	rdfs:label "profileApplication" ;
	rdfs:comment "A ProfileApplication that belongs to this Package. Based on the UML property 'Package-profileApplication' which is described as: References the ProfileApplications that indicate which profiles have been applied to the Package.."@en ;
	rdfs:domain uml-class:Package ;
	rdfs:range uml-class:ProfileApplication ;
	mms-ontology:umlPropertySource uml-property:Package-profileApplication .

mms-property:qualifierPropertyFromReadLinkObjectEndQualifierAction a mms-ontology:UmlObjectProperty ;
	mms-ontology:key "qualifierIds" ;
	rdfs:label "qualifierPropertyFromReadLinkObjectEndQualifierAction" ;
	rdfs:comment "The Property that is the qualifier of this ReadLinkObjectEndQualifierAction. Based on the UML property 'ReadLinkObjectEndQualifierAction-qualifier' which is described as: The qualifier Property to be read.."@en ;
	rdfs:domain uml-class:ReadLinkObjectEndQualifierAction ;
	rdfs:range uml-class:Property ;
	mms-ontology:umlPropertySource uml-property:ReadLinkObjectEndQualifierAction-qualifier .

mms-property:qualifierPropertyFromQualifierValue a mms-ontology:UmlObjectProperty ;
	mms-ontology:key "qualifierIds" ;
	rdfs:label "qualifierPropertyFromQualifierValue" ;
	rdfs:comment "The Property that is the qualifier of this QualifierValue. Based on the UML property 'QualifierValue-qualifier' which is described as: The qualifier Property for which the value is to be specified.."@en ;
	rdfs:domain uml-class:QualifierValue ;
	rdfs:range uml-class:Property ;
	mms-ontology:umlPropertySource uml-property:QualifierValue-qualifier .

mms-property:qualifierPropertyFromProperty a mms-ontology:UmlObjectProperty ;
	mms-ontology:key "qualifierIds" ;
	rdfs:label "qualifierPropertyFromProperty" ;
	rdfs:comment "A Property that is the qualifier of this Property. Based on the UML property 'Property-qualifier' which is described as: An optional list of ordered qualifier attributes for the end.."@en ;
	rdfs:domain uml-class:Property ;
	rdfs:range uml-class:Property ;
	mms-ontology:umlPropertySource uml-property:Property-qualifier .

mms-property:qualifierQualifierValue a mms-ontology:UmlObjectProperty ;
	mms-ontology:key "qualifierIds" ;
	rdfs:label "qualifierQualifierValue" ;
	rdfs:comment "A QualifierValue that is the qualifier of this LinkEndData. Based on the UML property 'LinkEndData-qualifier' which is described as: A set of QualifierValues used to provide values for the qualifiers of the end.."@en ;
	rdfs:domain uml-class:LinkEndData ;
	rdfs:range uml-class:QualifierValue ;
	mms-ontology:umlPropertySource uml-property:LinkEndData-qualifier .

mms-property:receiveEventMessageEnd a mms-ontology:UmlObjectProperty ;
	mms-ontology:key "receiveEventId" ;
	rdfs:label "receiveEventMessageEnd" ;
	rdfs:comment "The MessageEnd that is the receiveEvent of this Message. Based on the UML property 'Message-receiveEvent' which is described as: References the Receiving of the Message.."@en ;
	rdfs:domain uml-class:Message ;
	rdfs:range uml-class:MessageEnd ;
	mms-ontology:umlPropertySource uml-property:Message-receiveEvent .

mms-property:redefinedOperation a mms-ontology:UmlObjectProperty ;
	mms-ontology:key "redefinedOperationIds" ;
	rdfs:label "redefinedOperation" ;
	rdfs:comment "A Operation that belongs to this Operation. Based on the UML property 'Operation-redefinedOperation' which is described as: The Operations that are redefined by this Operation.."@en ;
	rdfs:domain uml-class:Operation ;
	rdfs:range uml-class:Operation ;
	mms-ontology:umlPropertySource uml-property:Operation-redefinedOperation .

mms-property:redefinedProperty a mms-ontology:UmlObjectProperty ;
	mms-ontology:key "redefinedPropertyIds" ;
	rdfs:label "redefinedProperty" ;
	rdfs:comment "A Property that belongs to this Property. Based on the UML property 'Property-redefinedProperty' which is described as: The properties that are redefined by this property, if any.."@en ;
	rdfs:domain uml-class:Property ;
	rdfs:range uml-class:Property ;
	mms-ontology:umlPropertySource uml-property:Property-redefinedProperty .

mms-property:regionAsInputExpansionRegion a mms-ontology:UmlObjectProperty ;
	mms-ontology:key "regionAsInputId" ;
	rdfs:label "regionAsInputExpansionRegion" ;
	rdfs:comment "The ExpansionRegion that is the regionAsInput of this ExpansionNode. Based on the UML property 'ExpansionNode-regionAsInput' which is described as: The ExpansionRegion for which the ExpansionNode is an input.."@en ;
	rdfs:domain uml-class:ExpansionNode ;
	rdfs:range uml-class:ExpansionRegion ;
	mms-ontology:umlPropertySource uml-property:ExpansionNode-regionAsInput .

mms-property:regionFromStateMachine a mms-ontology:UmlObjectProperty ;
	mms-ontology:key "regionIds" ;
	rdfs:label "regionFromStateMachine" ;
	rdfs:comment "A Region that belongs to this StateMachine. Based on the UML property 'StateMachine-region' which is described as: The Regions owned directly by the StateMachine.."@en ;
	rdfs:domain uml-class:StateMachine ;
	rdfs:range uml-class:Region ;
	mms-ontology:umlPropertySource uml-property:StateMachine-region .

mms-property:regionFromState a mms-ontology:UmlObjectProperty ;
	mms-ontology:key "regionIds" ;
	rdfs:label "regionFromState" ;
	rdfs:comment "A Region that belongs to this State. Based on the UML property 'State-region' which is described as: The Regions owned directly by the State.."@en ;
	rdfs:domain uml-class:State ;
	rdfs:range uml-class:Region ;
	mms-ontology:umlPropertySource uml-property:State-region .

mms-property:representsElement a mms-ontology:UmlObjectProperty ;
	mms-ontology:key "representsId" ;
	rdfs:label "representsElement" ;
	rdfs:comment "The Element that is the represents of this ActivityPartition. Based on the UML property 'ActivityPartition-represents' which is described as: An Element represented by the functionality modeled within the ActivityPartition.."@en ;
	rdfs:domain uml-class:ActivityPartition ;
	rdfs:range uml-class:Element ;
	mms-ontology:umlPropertySource uml-property:ActivityPartition-represents .

mms-property:representsConnectableElement a mms-ontology:UmlObjectProperty ;
	mms-ontology:key "representsId" ;
	rdfs:label "representsConnectableElement" ;
	rdfs:comment "The ConnectableElement that is the represents of this Lifeline. Based on the UML property 'Lifeline-represents' which is described as: References the ConnectableElement within the classifier that contains the enclosing interaction.."@en ;
	rdfs:domain uml-class:Lifeline ;
	rdfs:range uml-class:ConnectableElement ;
	mms-ontology:umlPropertySource uml-property:Lifeline-represents .

mms-property:resultParameter a mms-ontology:UmlObjectProperty ;
	mms-ontology:key "resultId" ;
	rdfs:label "resultParameter" ;
	rdfs:comment "The Parameter that is the result of this OpaqueExpression. Based on the UML property 'OpaqueExpression-result' which is described as: If an OpaqueExpression is specified using a UML Behavior, then this refers to the single required return Parameter of that Behavior. When the Behavior completes execution, the values on this Parameter give the result of evaluating the OpaqueExpression.."@en ;
	rdfs:domain uml-class:OpaqueExpression ;
	rdfs:range uml-class:Parameter ;
	mms-ontology:umlPropertySource uml-property:OpaqueExpression-result .

mms-property:resultOutputPinFromReadSelfAction a mms-ontology:UmlObjectProperty ;
	mms-ontology:key "resultId" ;
	rdfs:label "resultOutputPinFromReadSelfAction" ;
	rdfs:comment "The OutputPin that is the result of this ReadSelfAction. Based on the UML property 'ReadSelfAction-result' which is described as: The OutputPin on which the context object is placed.."@en ;
	rdfs:domain uml-class:ReadSelfAction ;
	rdfs:range uml-class:OutputPin ;
	mms-ontology:umlPropertySource uml-property:ReadSelfAction-result .

mms-property:resultOutputPinFromConditionalNode a mms-ontology:UmlObjectProperty ;
	mms-ontology:key "resultId" ;
	rdfs:label "resultOutputPinFromConditionalNode" ;
	rdfs:comment "The OutputPin that is the result of this ConditionalNode. Based on the UML property 'ConditionalNode-result' which is described as: The OutputPins that onto which are moved values from the bodyOutputs of the Clause selected for execution.."@en ;
	rdfs:domain uml-class:ConditionalNode ;
	rdfs:range uml-class:OutputPin ;
	mms-ontology:umlPropertySource uml-property:ConditionalNode-result .

mms-property:resultOutputPinFromReadIsClassifiedObjectAction a mms-ontology:UmlObjectProperty ;
	mms-ontology:key "resultId" ;
	rdfs:label "resultOutputPinFromReadIsClassifiedObjectAction" ;
	rdfs:comment "The OutputPin that is the result of this ReadIsClassifiedObjectAction. Based on the UML property 'ReadIsClassifiedObjectAction-result' which is described as: The OutputPin that holds the Boolean result of the test.."@en ;
	rdfs:domain uml-class:ReadIsClassifiedObjectAction ;
	rdfs:range uml-class:OutputPin ;
	mms-ontology:umlPropertySource uml-property:ReadIsClassifiedObjectAction-result .

mms-property:resultOutputPinFromCallAction a mms-ontology:UmlObjectProperty ;
	mms-ontology:key "resultId" ;
	rdfs:label "resultOutputPinFromCallAction" ;
	rdfs:comment "The OutputPin that is the result of this CallAction. Based on the UML property 'CallAction-result' which is described as: The OutputPins on which the reply values from the invocation are placed (if the call is synchronous).."@en ;
	rdfs:domain uml-class:CallAction ;
	rdfs:range uml-class:OutputPin ;
	mms-ontology:umlPropertySource uml-property:CallAction-result .

mms-property:resultOutputPinFromLoopNode a mms-ontology:UmlObjectProperty ;
	mms-ontology:key "resultId" ;
	rdfs:label "resultOutputPinFromLoopNode" ;
	rdfs:comment "The OutputPin that is the result of this LoopNode. Based on the UML property 'LoopNode-result' which is described as: A list of OutputPins that receive the loopVariable values after the last iteration of the loop and constitute the output of the LoopNode.."@en ;
	rdfs:domain uml-class:LoopNode ;
	rdfs:range uml-class:OutputPin ;
	mms-ontology:umlPropertySource uml-property:LoopNode-result .

mms-property:resultOutputPinFromWriteStructuralFeatureAction a mms-ontology:UmlObjectProperty ;
	mms-ontology:key "resultId" ;
	rdfs:label "resultOutputPinFromWriteStructuralFeatureAction" ;
	rdfs:comment "The OutputPin that is the result of this WriteStructuralFeatureAction. Based on the UML property 'WriteStructuralFeatureAction-result' which is described as: The OutputPin on which is put the input object as modified by the WriteStructuralFeatureAction.."@en ;
	rdfs:domain uml-class:WriteStructuralFeatureAction ;
	rdfs:range uml-class:OutputPin ;
	mms-ontology:umlPropertySource uml-property:WriteStructuralFeatureAction-result .

mms-property:resultOutputPinFromReadStructuralFeatureAction a mms-ontology:UmlObjectProperty ;
	mms-ontology:key "resultId" ;
	rdfs:label "resultOutputPinFromReadStructuralFeatureAction" ;
	rdfs:comment "The OutputPin that is the result of this ReadStructuralFeatureAction. Based on the UML property 'ReadStructuralFeatureAction-result' which is described as: The OutputPin on which the result values are placed.."@en ;
	rdfs:domain uml-class:ReadStructuralFeatureAction ;
	rdfs:range uml-class:OutputPin ;
	mms-ontology:umlPropertySource uml-property:ReadStructuralFeatureAction-result .

mms-property:resultOutputPinFromReadLinkAction a mms-ontology:UmlObjectProperty ;
	mms-ontology:key "resultId" ;
	rdfs:label "resultOutputPinFromReadLinkAction" ;
	rdfs:comment "The OutputPin that is the result of this ReadLinkAction. Based on the UML property 'ReadLinkAction-result' which is described as: The OutputPin on which the objects retrieved from the &#34;open&#34; end of those links whose values on other ends are given by the endData.."@en ;
	rdfs:domain uml-class:ReadLinkAction ;
	rdfs:range uml-class:OutputPin ;
	mms-ontology:umlPropertySource uml-property:ReadLinkAction-result .

mms-property:resultOutputPinFromCreateObjectAction a mms-ontology:UmlObjectProperty ;
	mms-ontology:key "resultId" ;
	rdfs:label "resultOutputPinFromCreateObjectAction" ;
	rdfs:comment "The OutputPin that is the result of this CreateObjectAction. Based on the UML property 'CreateObjectAction-result' which is described as: The OutputPin on which the newly created object is placed.."@en ;
	rdfs:domain uml-class:CreateObjectAction ;
	rdfs:range uml-class:OutputPin ;
	mms-ontology:umlPropertySource uml-property:CreateObjectAction-result .

mms-property:resultOutputPinFromAcceptEventAction a mms-ontology:UmlObjectProperty ;
	mms-ontology:key "resultId" ;
	rdfs:label "resultOutputPinFromAcceptEventAction" ;
	rdfs:comment "The OutputPin that is the result of this AcceptEventAction. Based on the UML property 'AcceptEventAction-result' which is described as: OutputPins holding the values received from an Event occurrence.."@en ;
	rdfs:domain uml-class:AcceptEventAction ;
	rdfs:range uml-class:OutputPin ;
	mms-ontology:umlPropertySource uml-property:AcceptEventAction-result .

mms-property:resultOutputPinFromClearStructuralFeatureAction a mms-ontology:UmlObjectProperty ;
	mms-ontology:key "resultId" ;
	rdfs:label "resultOutputPinFromClearStructuralFeatureAction" ;
	rdfs:comment "The OutputPin that is the result of this ClearStructuralFeatureAction. Based on the UML property 'ClearStructuralFeatureAction-result' which is described as: The OutputPin on which is put the input object as modified by the ClearStructuralFeatureAction.."@en ;
	rdfs:domain uml-class:ClearStructuralFeatureAction ;
	rdfs:range uml-class:OutputPin ;
	mms-ontology:umlPropertySource uml-property:ClearStructuralFeatureAction-result .

mms-property:resultOutputPinFromReadLinkObjectEndAction a mms-ontology:UmlObjectProperty ;
	mms-ontology:key "resultId" ;
	rdfs:label "resultOutputPinFromReadLinkObjectEndAction" ;
	rdfs:comment "The OutputPin that is the result of this ReadLinkObjectEndAction. Based on the UML property 'ReadLinkObjectEndAction-result' which is described as: The OutputPin where the result value is placed.."@en ;
	rdfs:domain uml-class:ReadLinkObjectEndAction ;
	rdfs:range uml-class:OutputPin ;
	mms-ontology:umlPropertySource uml-property:ReadLinkObjectEndAction-result .

mms-property:resultOutputPinFromReduceAction a mms-ontology:UmlObjectProperty ;
	mms-ontology:key "resultId" ;
	rdfs:label "resultOutputPinFromReduceAction" ;
	rdfs:comment "The OutputPin that is the result of this ReduceAction. Based on the UML property 'ReduceAction-result' which is described as: The output pin on which the result value is placed.."@en ;
	rdfs:domain uml-class:ReduceAction ;
	rdfs:range uml-class:OutputPin ;
	mms-ontology:umlPropertySource uml-property:ReduceAction-result .

mms-property:resultOutputPinFromReadLinkObjectEndQualifierAction a mms-ontology:UmlObjectProperty ;
	mms-ontology:key "resultId" ;
	rdfs:label "resultOutputPinFromReadLinkObjectEndQualifierAction" ;
	rdfs:comment "The OutputPin that is the result of this ReadLinkObjectEndQualifierAction. Based on the UML property 'ReadLinkObjectEndQualifierAction-result' which is described as: The OutputPin where the result value is placed.."@en ;
	rdfs:domain uml-class:ReadLinkObjectEndQualifierAction ;
	rdfs:range uml-class:OutputPin ;
	mms-ontology:umlPropertySource uml-property:ReadLinkObjectEndQualifierAction-result .

mms-property:resultOutputPinFromReadExtentAction a mms-ontology:UmlObjectProperty ;
	mms-ontology:key "resultId" ;
	rdfs:label "resultOutputPinFromReadExtentAction" ;
	rdfs:comment "The OutputPin that is the result of this ReadExtentAction. Based on the UML property 'ReadExtentAction-result' which is described as: The OutputPin on which the Classifier instances are placed.."@en ;
	rdfs:domain uml-class:ReadExtentAction ;
	rdfs:range uml-class:OutputPin ;
	mms-ontology:umlPropertySource uml-property:ReadExtentAction-result .

mms-property:resultOutputPinFromTestIdentityAction a mms-ontology:UmlObjectProperty ;
	mms-ontology:key "resultId" ;
	rdfs:label "resultOutputPinFromTestIdentityAction" ;
	rdfs:comment "The OutputPin that is the result of this TestIdentityAction. Based on the UML property 'TestIdentityAction-result' which is described as: The OutputPin whose Boolean value indicates whether the two input objects are identical.."@en ;
	rdfs:domain uml-class:TestIdentityAction ;
	rdfs:range uml-class:OutputPin ;
	mms-ontology:umlPropertySource uml-property:TestIdentityAction-result .

mms-property:resultOutputPinFromReadVariableAction a mms-ontology:UmlObjectProperty ;
	mms-ontology:key "resultId" ;
	rdfs:label "resultOutputPinFromReadVariableAction" ;
	rdfs:comment "The OutputPin that is the result of this ReadVariableAction. Based on the UML property 'ReadVariableAction-result' which is described as: The OutputPin on which the result values are placed.."@en ;
	rdfs:domain uml-class:ReadVariableAction ;
	rdfs:range uml-class:OutputPin ;
	mms-ontology:umlPropertySource uml-property:ReadVariableAction-result .

mms-property:resultOutputPinFromCreateLinkObjectAction a mms-ontology:UmlObjectProperty ;
	mms-ontology:key "resultId" ;
	rdfs:label "resultOutputPinFromCreateLinkObjectAction" ;
	rdfs:comment "The OutputPin that is the result of this CreateLinkObjectAction. Based on the UML property 'CreateLinkObjectAction-result' which is described as: The output pin on which the newly created link object is placed.."@en ;
	rdfs:domain uml-class:CreateLinkObjectAction ;
	rdfs:range uml-class:OutputPin ;
	mms-ontology:umlPropertySource uml-property:CreateLinkObjectAction-result .

mms-property:resultOutputPinFromUnmarshallAction a mms-ontology:UmlObjectProperty ;
	mms-ontology:key "resultId" ;
	rdfs:label "resultOutputPinFromUnmarshallAction" ;
	rdfs:comment "The OutputPin that is the result of this UnmarshallAction. Based on the UML property 'UnmarshallAction-result' which is described as: The OutputPins on which are placed the values of the StructuralFeatures of the input object.."@en ;
	rdfs:domain uml-class:UnmarshallAction ;
	rdfs:range uml-class:OutputPin ;
	mms-ontology:umlPropertySource uml-property:UnmarshallAction-result .

mms-property:resultOutputPinFromValueSpecificationAction a mms-ontology:UmlObjectProperty ;
	mms-ontology:key "resultId" ;
	rdfs:label "resultOutputPinFromValueSpecificationAction" ;
	rdfs:comment "The OutputPin that is the result of this ValueSpecificationAction. Based on the UML property 'ValueSpecificationAction-result' which is described as: The OutputPin on which the result value is placed.."@en ;
	rdfs:domain uml-class:ValueSpecificationAction ;
	rdfs:range uml-class:OutputPin ;
	mms-ontology:umlPropertySource uml-property:ValueSpecificationAction-result .

mms-property:resultParameter a mms-ontology:UmlObjectProperty ;
	mms-ontology:key "resultIds" ;
	rdfs:label "resultParameter" ;
	rdfs:comment "The Parameter that is the result of this OpaqueExpression. Based on the UML property 'OpaqueExpression-result' which is described as: If an OpaqueExpression is specified using a UML Behavior, then this refers to the single required return Parameter of that Behavior. When the Behavior completes execution, the values on this Parameter give the result of evaluating the OpaqueExpression.."@en ;
	rdfs:domain uml-class:OpaqueExpression ;
	rdfs:range uml-class:Parameter ;
	mms-ontology:umlPropertySource uml-property:OpaqueExpression-result .

mms-property:resultOutputPinFromReadSelfAction a mms-ontology:UmlObjectProperty ;
	mms-ontology:key "resultIds" ;
	rdfs:label "resultOutputPinFromReadSelfAction" ;
	rdfs:comment "The OutputPin that is the result of this ReadSelfAction. Based on the UML property 'ReadSelfAction-result' which is described as: The OutputPin on which the context object is placed.."@en ;
	rdfs:domain uml-class:ReadSelfAction ;
	rdfs:range uml-class:OutputPin ;
	mms-ontology:umlPropertySource uml-property:ReadSelfAction-result .

mms-property:resultOutputPinFromConditionalNode a mms-ontology:UmlObjectProperty ;
	mms-ontology:key "resultIds" ;
	rdfs:label "resultOutputPinFromConditionalNode" ;
	rdfs:comment "A OutputPin that is the result of this ConditionalNode. Based on the UML property 'ConditionalNode-result' which is described as: The OutputPins that onto which are moved values from the bodyOutputs of the Clause selected for execution.."@en ;
	rdfs:domain uml-class:ConditionalNode ;
	rdfs:range uml-class:OutputPin ;
	mms-ontology:umlPropertySource uml-property:ConditionalNode-result .

mms-property:resultOutputPinFromReadIsClassifiedObjectAction a mms-ontology:UmlObjectProperty ;
	mms-ontology:key "resultIds" ;
	rdfs:label "resultOutputPinFromReadIsClassifiedObjectAction" ;
	rdfs:comment "The OutputPin that is the result of this ReadIsClassifiedObjectAction. Based on the UML property 'ReadIsClassifiedObjectAction-result' which is described as: The OutputPin that holds the Boolean result of the test.."@en ;
	rdfs:domain uml-class:ReadIsClassifiedObjectAction ;
	rdfs:range uml-class:OutputPin ;
	mms-ontology:umlPropertySource uml-property:ReadIsClassifiedObjectAction-result .

mms-property:resultOutputPinFromCallAction a mms-ontology:UmlObjectProperty ;
	mms-ontology:key "resultIds" ;
	rdfs:label "resultOutputPinFromCallAction" ;
	rdfs:comment "A OutputPin that is the result of this CallAction. Based on the UML property 'CallAction-result' which is described as: The OutputPins on which the reply values from the invocation are placed (if the call is synchronous).."@en ;
	rdfs:domain uml-class:CallAction ;
	rdfs:range uml-class:OutputPin ;
	mms-ontology:umlPropertySource uml-property:CallAction-result .

mms-property:resultOutputPinFromLoopNode a mms-ontology:UmlObjectProperty ;
	mms-ontology:key "resultIds" ;
	rdfs:label "resultOutputPinFromLoopNode" ;
	rdfs:comment "A OutputPin that is the result of this LoopNode. Based on the UML property 'LoopNode-result' which is described as: A list of OutputPins that receive the loopVariable values after the last iteration of the loop and constitute the output of the LoopNode.."@en ;
	rdfs:domain uml-class:LoopNode ;
	rdfs:range uml-class:OutputPin ;
	mms-ontology:umlPropertySource uml-property:LoopNode-result .

mms-property:resultOutputPinFromWriteStructuralFeatureAction a mms-ontology:UmlObjectProperty ;
	mms-ontology:key "resultIds" ;
	rdfs:label "resultOutputPinFromWriteStructuralFeatureAction" ;
	rdfs:comment "The OutputPin that is the result of this WriteStructuralFeatureAction. Based on the UML property 'WriteStructuralFeatureAction-result' which is described as: The OutputPin on which is put the input object as modified by the WriteStructuralFeatureAction.."@en ;
	rdfs:domain uml-class:WriteStructuralFeatureAction ;
	rdfs:range uml-class:OutputPin ;
	mms-ontology:umlPropertySource uml-property:WriteStructuralFeatureAction-result .

mms-property:resultOutputPinFromReadStructuralFeatureAction a mms-ontology:UmlObjectProperty ;
	mms-ontology:key "resultIds" ;
	rdfs:label "resultOutputPinFromReadStructuralFeatureAction" ;
	rdfs:comment "The OutputPin that is the result of this ReadStructuralFeatureAction. Based on the UML property 'ReadStructuralFeatureAction-result' which is described as: The OutputPin on which the result values are placed.."@en ;
	rdfs:domain uml-class:ReadStructuralFeatureAction ;
	rdfs:range uml-class:OutputPin ;
	mms-ontology:umlPropertySource uml-property:ReadStructuralFeatureAction-result .

mms-property:resultOutputPinFromReadLinkAction a mms-ontology:UmlObjectProperty ;
	mms-ontology:key "resultIds" ;
	rdfs:label "resultOutputPinFromReadLinkAction" ;
	rdfs:comment "The OutputPin that is the result of this ReadLinkAction. Based on the UML property 'ReadLinkAction-result' which is described as: The OutputPin on which the objects retrieved from the &#34;open&#34; end of those links whose values on other ends are given by the endData.."@en ;
	rdfs:domain uml-class:ReadLinkAction ;
	rdfs:range uml-class:OutputPin ;
	mms-ontology:umlPropertySource uml-property:ReadLinkAction-result .

mms-property:resultOutputPinFromCreateObjectAction a mms-ontology:UmlObjectProperty ;
	mms-ontology:key "resultIds" ;
	rdfs:label "resultOutputPinFromCreateObjectAction" ;
	rdfs:comment "The OutputPin that is the result of this CreateObjectAction. Based on the UML property 'CreateObjectAction-result' which is described as: The OutputPin on which the newly created object is placed.."@en ;
	rdfs:domain uml-class:CreateObjectAction ;
	rdfs:range uml-class:OutputPin ;
	mms-ontology:umlPropertySource uml-property:CreateObjectAction-result .

mms-property:resultOutputPinFromAcceptEventAction a mms-ontology:UmlObjectProperty ;
	mms-ontology:key "resultIds" ;
	rdfs:label "resultOutputPinFromAcceptEventAction" ;
	rdfs:comment "A OutputPin that is the result of this AcceptEventAction. Based on the UML property 'AcceptEventAction-result' which is described as: OutputPins holding the values received from an Event occurrence.."@en ;
	rdfs:domain uml-class:AcceptEventAction ;
	rdfs:range uml-class:OutputPin ;
	mms-ontology:umlPropertySource uml-property:AcceptEventAction-result .

mms-property:resultOutputPinFromClearStructuralFeatureAction a mms-ontology:UmlObjectProperty ;
	mms-ontology:key "resultIds" ;
	rdfs:label "resultOutputPinFromClearStructuralFeatureAction" ;
	rdfs:comment "The OutputPin that is the result of this ClearStructuralFeatureAction. Based on the UML property 'ClearStructuralFeatureAction-result' which is described as: The OutputPin on which is put the input object as modified by the ClearStructuralFeatureAction.."@en ;
	rdfs:domain uml-class:ClearStructuralFeatureAction ;
	rdfs:range uml-class:OutputPin ;
	mms-ontology:umlPropertySource uml-property:ClearStructuralFeatureAction-result .

mms-property:resultOutputPinFromReadLinkObjectEndAction a mms-ontology:UmlObjectProperty ;
	mms-ontology:key "resultIds" ;
	rdfs:label "resultOutputPinFromReadLinkObjectEndAction" ;
	rdfs:comment "The OutputPin that is the result of this ReadLinkObjectEndAction. Based on the UML property 'ReadLinkObjectEndAction-result' which is described as: The OutputPin where the result value is placed.."@en ;
	rdfs:domain uml-class:ReadLinkObjectEndAction ;
	rdfs:range uml-class:OutputPin ;
	mms-ontology:umlPropertySource uml-property:ReadLinkObjectEndAction-result .

mms-property:resultOutputPinFromReduceAction a mms-ontology:UmlObjectProperty ;
	mms-ontology:key "resultIds" ;
	rdfs:label "resultOutputPinFromReduceAction" ;
	rdfs:comment "The OutputPin that is the result of this ReduceAction. Based on the UML property 'ReduceAction-result' which is described as: The output pin on which the result value is placed.."@en ;
	rdfs:domain uml-class:ReduceAction ;
	rdfs:range uml-class:OutputPin ;
	mms-ontology:umlPropertySource uml-property:ReduceAction-result .

mms-property:resultOutputPinFromReadLinkObjectEndQualifierAction a mms-ontology:UmlObjectProperty ;
	mms-ontology:key "resultIds" ;
	rdfs:label "resultOutputPinFromReadLinkObjectEndQualifierAction" ;
	rdfs:comment "The OutputPin that is the result of this ReadLinkObjectEndQualifierAction. Based on the UML property 'ReadLinkObjectEndQualifierAction-result' which is described as: The OutputPin where the result value is placed.."@en ;
	rdfs:domain uml-class:ReadLinkObjectEndQualifierAction ;
	rdfs:range uml-class:OutputPin ;
	mms-ontology:umlPropertySource uml-property:ReadLinkObjectEndQualifierAction-result .

mms-property:resultOutputPinFromReadExtentAction a mms-ontology:UmlObjectProperty ;
	mms-ontology:key "resultIds" ;
	rdfs:label "resultOutputPinFromReadExtentAction" ;
	rdfs:comment "The OutputPin that is the result of this ReadExtentAction. Based on the UML property 'ReadExtentAction-result' which is described as: The OutputPin on which the Classifier instances are placed.."@en ;
	rdfs:domain uml-class:ReadExtentAction ;
	rdfs:range uml-class:OutputPin ;
	mms-ontology:umlPropertySource uml-property:ReadExtentAction-result .

mms-property:resultOutputPinFromTestIdentityAction a mms-ontology:UmlObjectProperty ;
	mms-ontology:key "resultIds" ;
	rdfs:label "resultOutputPinFromTestIdentityAction" ;
	rdfs:comment "The OutputPin that is the result of this TestIdentityAction. Based on the UML property 'TestIdentityAction-result' which is described as: The OutputPin whose Boolean value indicates whether the two input objects are identical.."@en ;
	rdfs:domain uml-class:TestIdentityAction ;
	rdfs:range uml-class:OutputPin ;
	mms-ontology:umlPropertySource uml-property:TestIdentityAction-result .

mms-property:resultOutputPinFromReadVariableAction a mms-ontology:UmlObjectProperty ;
	mms-ontology:key "resultIds" ;
	rdfs:label "resultOutputPinFromReadVariableAction" ;
	rdfs:comment "The OutputPin that is the result of this ReadVariableAction. Based on the UML property 'ReadVariableAction-result' which is described as: The OutputPin on which the result values are placed.."@en ;
	rdfs:domain uml-class:ReadVariableAction ;
	rdfs:range uml-class:OutputPin ;
	mms-ontology:umlPropertySource uml-property:ReadVariableAction-result .

mms-property:resultOutputPinFromCreateLinkObjectAction a mms-ontology:UmlObjectProperty ;
	mms-ontology:key "resultIds" ;
	rdfs:label "resultOutputPinFromCreateLinkObjectAction" ;
	rdfs:comment "The OutputPin that is the result of this CreateLinkObjectAction. Based on the UML property 'CreateLinkObjectAction-result' which is described as: The output pin on which the newly created link object is placed.."@en ;
	rdfs:domain uml-class:CreateLinkObjectAction ;
	rdfs:range uml-class:OutputPin ;
	mms-ontology:umlPropertySource uml-property:CreateLinkObjectAction-result .

mms-property:resultOutputPinFromUnmarshallAction a mms-ontology:UmlObjectProperty ;
	mms-ontology:key "resultIds" ;
	rdfs:label "resultOutputPinFromUnmarshallAction" ;
	rdfs:comment "A OutputPin that is the result of this UnmarshallAction. Based on the UML property 'UnmarshallAction-result' which is described as: The OutputPins on which are placed the values of the StructuralFeatures of the input object.."@en ;
	rdfs:domain uml-class:UnmarshallAction ;
	rdfs:range uml-class:OutputPin ;
	mms-ontology:umlPropertySource uml-property:UnmarshallAction-result .

mms-property:resultOutputPinFromValueSpecificationAction a mms-ontology:UmlObjectProperty ;
	mms-ontology:key "resultIds" ;
	rdfs:label "resultOutputPinFromValueSpecificationAction" ;
	rdfs:comment "The OutputPin that is the result of this ValueSpecificationAction. Based on the UML property 'ValueSpecificationAction-result' which is described as: The OutputPin on which the result value is placed.."@en ;
	rdfs:domain uml-class:ValueSpecificationAction ;
	rdfs:range uml-class:OutputPin ;
	mms-ontology:umlPropertySource uml-property:ValueSpecificationAction-result .

mms-property:roleConnectableElementFromStructuredClassifier a mms-ontology:UmlObjectProperty ;
	mms-ontology:key "roleId" ;
	rdfs:label "roleConnectableElementFromStructuredClassifier" ;
	rdfs:comment "The ConnectableElement that is the role of this StructuredClassifier. Based on the UML property 'StructuredClassifier-role' which is described as: The roles that instances may play in this StructuredClassifier.."@en ;
	rdfs:domain uml-class:StructuredClassifier ;
	rdfs:range uml-class:ConnectableElement ;
	mms-ontology:umlPropertySource uml-property:StructuredClassifier-role .

mms-property:roleConnectableElementFromConnectorEnd a mms-ontology:UmlObjectProperty ;
	mms-ontology:key "roleId" ;
	rdfs:label "roleConnectableElementFromConnectorEnd" ;
	rdfs:comment "The ConnectableElement that is the role of this ConnectorEnd. Based on the UML property 'ConnectorEnd-role' which is described as: The ConnectableElement attached at this ConnectorEnd. When an instance of the containing Classifier is created, a link may (depending on the multiplicities) be created to an instance of the Classifier that types this ConnectableElement.."@en ;
	rdfs:domain uml-class:ConnectorEnd ;
	rdfs:range uml-class:ConnectableElement ;
	mms-ontology:umlPropertySource uml-property:ConnectorEnd-role .

mms-property:sendEventMessageEnd a mms-ontology:UmlObjectProperty ;
	mms-ontology:key "sendEventId" ;
	rdfs:label "sendEventMessageEnd" ;
	rdfs:comment "The MessageEnd that is the sendEvent of this Message. Based on the UML property 'Message-sendEvent' which is described as: References the Sending of the Message.."@en ;
	rdfs:domain uml-class:Message ;
	rdfs:range uml-class:MessageEnd ;
	mms-ontology:umlPropertySource uml-property:Message-sendEvent .

mms-property:setupPart a mms-ontology:UmlObjectProperty ;
	mms-ontology:key "setupPartIds" ;
	rdfs:label "setupPart" ;
	rdfs:comment "A ExecutableNode that is the setupPart of this LoopNode. Based on the UML property 'LoopNode-setupPart' which is described as: The set of ExecutableNodes executed before the first iteration of the loop, in order to initialize values or perform other setup computations.."@en ;
	rdfs:domain uml-class:LoopNode ;
	rdfs:range uml-class:ExecutableNode ;
	mms-ontology:umlPropertySource uml-property:LoopNode-setupPart .

mms-property:signalFromSendSignalAction a mms-ontology:UmlObjectProperty ;
	mms-ontology:key "signalId" ;
	rdfs:label "signalFromSendSignalAction" ;
	rdfs:comment "The Signal that belongs to this SendSignalAction. Based on the UML property 'SendSignalAction-signal' which is described as: The Signal whose instance is transmitted to the target.."@en ;
	rdfs:domain uml-class:SendSignalAction ;
	rdfs:range uml-class:Signal ;
	mms-ontology:umlPropertySource uml-property:SendSignalAction-signal .

mms-property:signalFromReception a mms-ontology:UmlObjectProperty ;
	mms-ontology:key "signalId" ;
	rdfs:label "signalFromReception" ;
	rdfs:comment "The Signal that belongs to this Reception. Based on the UML property 'Reception-signal' which is described as: The Signal that this Reception handles.."@en ;
	rdfs:domain uml-class:Reception ;
	rdfs:range uml-class:Signal ;
	mms-ontology:umlPropertySource uml-property:Reception-signal .

mms-property:signalFromSignalEvent a mms-ontology:UmlObjectProperty ;
	mms-ontology:key "signalId" ;
	rdfs:label "signalFromSignalEvent" ;
	rdfs:comment "The Signal that belongs to this SignalEvent. Based on the UML property 'SignalEvent-signal' which is described as: The specific Signal that is associated with this SignalEvent.."@en ;
	rdfs:domain uml-class:SignalEvent ;
	rdfs:range uml-class:Signal ;
	mms-ontology:umlPropertySource uml-property:SignalEvent-signal .

mms-property:signalFromBroadcastSignalAction a mms-ontology:UmlObjectProperty ;
	mms-ontology:key "signalId" ;
	rdfs:label "signalFromBroadcastSignalAction" ;
	rdfs:comment "The Signal that belongs to this BroadcastSignalAction. Based on the UML property 'BroadcastSignalAction-signal' which is described as: The Signal whose instances are to be sent.."@en ;
	rdfs:domain uml-class:BroadcastSignalAction ;
	rdfs:range uml-class:Signal ;
	mms-ontology:umlPropertySource uml-property:BroadcastSignalAction-signal .

mms-property:signatureNamedElement a mms-ontology:UmlObjectProperty ;
	mms-ontology:key "signatureId" ;
	rdfs:label "signatureNamedElement" ;
	rdfs:comment "The NamedElement that is the signature of this Message. Based on the UML property 'Message-signature' which is described as: The signature of the Message is the specification of its content. It refers either an Operation or a Signal.."@en ;
	rdfs:domain uml-class:Message ;
	rdfs:range uml-class:NamedElement ;
	mms-ontology:umlPropertySource uml-property:Message-signature .

mms-property:signatureTemplateSignatureFromTemplateParameter a mms-ontology:UmlObjectProperty ;
	mms-ontology:key "signatureId" ;
	rdfs:label "signatureTemplateSignatureFromTemplateParameter" ;
	rdfs:comment "The TemplateSignature that is the signature of this TemplateParameter. Based on the UML property 'TemplateParameter-signature' which is described as: The TemplateSignature that owns this TemplateParameter.."@en ;
	rdfs:domain uml-class:TemplateParameter ;
	rdfs:range uml-class:TemplateSignature ;
	mms-ontology:umlPropertySource uml-property:TemplateParameter-signature .

mms-property:signatureTemplateSignatureFromTemplateBinding a mms-ontology:UmlObjectProperty ;
	mms-ontology:key "signatureId" ;
	rdfs:label "signatureTemplateSignatureFromTemplateBinding" ;
	rdfs:comment "The TemplateSignature that is the signature of this TemplateBinding. Based on the UML property 'TemplateBinding-signature' which is described as: The TemplateSignature for the template that is the target of this TemplateBinding.."@en ;
	rdfs:domain uml-class:TemplateBinding ;
	rdfs:range uml-class:TemplateSignature ;
	mms-ontology:umlPropertySource uml-property:TemplateBinding-signature .

mms-property:slot a mms-ontology:UmlObjectProperty ;
	mms-ontology:key "slotIds" ;
	rdfs:label "slot" ;
	rdfs:comment "A Slot that belongs to this InstanceSpecification. Based on the UML property 'InstanceSpecification-slot' which is described as: A Slot giving the value or values of a StructuralFeature of the instance. An InstanceSpecification can have one Slot per StructuralFeature of its Classifiers, including inherited features. It is not necessary to model a Slot for every StructuralFeature, in which case the InstanceSpecification is a partial description.."@en ;
	rdfs:domain uml-class:InstanceSpecification ;
	rdfs:range uml-class:Slot ;
	mms-ontology:umlPropertySource uml-property:InstanceSpecification-slot .

mms-property:sourceActivityNode a mms-ontology:UmlObjectProperty ;
	mms-ontology:key "sourceId" ;
	rdfs:label "sourceActivityNode" ;
	rdfs:comment "The ActivityNode that is the source of this ActivityEdge. Based on the UML property 'ActivityEdge-source' which is described as: The ActivityNode from which tokens are taken when they traverse the ActivityEdge.."@en ;
	rdfs:domain uml-class:ActivityEdge ;
	rdfs:range uml-class:ActivityNode ;
	mms-ontology:umlPropertySource uml-property:ActivityEdge-source .

mms-property:sourceVertex a mms-ontology:UmlObjectProperty ;
	mms-ontology:key "sourceId" ;
	rdfs:label "sourceVertex" ;
	rdfs:comment "The Vertex that is the source of this Transition. Based on the UML property 'Transition-source' which is described as: Designates the originating Vertex (State or Pseudostate) of the Transition.."@en ;
	rdfs:domain uml-class:Transition ;
	rdfs:range uml-class:Vertex ;
	mms-ontology:umlPropertySource uml-property:Transition-source .

mms-property:sourceElement a mms-ontology:UmlObjectProperty ;
	mms-ontology:key "sourceId" ;
	rdfs:label "sourceElement" ;
	rdfs:comment "The Element that is the source of this DirectedRelationship. Based on the UML property 'DirectedRelationship-source' which is described as: Specifies the source Element(s) of the DirectedRelationship.."@en ;
	rdfs:domain uml-class:DirectedRelationship ;
	rdfs:range uml-class:Element ;
	mms-ontology:umlPropertySource uml-property:DirectedRelationship-source .

mms-property:specificClassifier a mms-ontology:UmlObjectProperty ;
	mms-ontology:key "specificId" ;
	rdfs:label "specificClassifier" ;
	rdfs:comment "The Classifier that is the specific of this Generalization. Based on the UML property 'Generalization-specific' which is described as: The specializing Classifier in the Generalization relationship.."@en ;
	rdfs:domain uml-class:Generalization ;
	rdfs:range uml-class:Classifier ;
	mms-ontology:umlPropertySource uml-property:Generalization-specific .

mms-property:specificationDurationInterval a mms-ontology:UmlObjectProperty ;
	mms-ontology:key "specificationId" ;
	rdfs:label "specificationDurationInterval" ;
	rdfs:comment "The DurationInterval that is the specification of this DurationConstraint. Based on the UML property 'DurationConstraint-specification' which is described as: The DurationInterval constraining the duration.."@en ;
	rdfs:domain uml-class:DurationConstraint ;
	rdfs:range uml-class:DurationInterval ;
	mms-ontology:umlPropertySource uml-property:DurationConstraint-specification .

mms-property:specificationValueSpecificationFromConstraint a mms-ontology:UmlObjectProperty ;
	mms-ontology:key "specificationId" ;
	rdfs:label "specificationValueSpecificationFromConstraint" ;
	rdfs:comment "The ValueSpecification that is the specification of this Constraint. Based on the UML property 'Constraint-specification' which is described as: A condition that must be true when evaluated in order for the Constraint to be satisfied.."@en ;
	rdfs:domain uml-class:Constraint ;
	rdfs:range uml-class:ValueSpecification ;
	mms-ontology:umlPropertySource uml-property:Constraint-specification .

mms-property:specificationValueSpecificationFromInstanceSpecification a mms-ontology:UmlObjectProperty ;
	mms-ontology:key "specificationId" ;
	rdfs:label "specificationValueSpecificationFromInstanceSpecification" ;
	rdfs:comment "The ValueSpecification that is the specification of this InstanceSpecification. Based on the UML property 'InstanceSpecification-specification' which is described as: A specification of how to compute, derive, or construct the instance.."@en ;
	rdfs:domain uml-class:InstanceSpecification ;
	rdfs:range uml-class:ValueSpecification ;
	mms-ontology:umlPropertySource uml-property:InstanceSpecification-specification .

mms-property:specificationTimeInterval a mms-ontology:UmlObjectProperty ;
	mms-ontology:key "specificationId" ;
	rdfs:label "specificationTimeInterval" ;
	rdfs:comment "The TimeInterval that is the specification of this TimeConstraint. Based on the UML property 'TimeConstraint-specification' which is described as: TheTimeInterval constraining the duration.."@en ;
	rdfs:domain uml-class:TimeConstraint ;
	rdfs:range uml-class:TimeInterval ;
	mms-ontology:umlPropertySource uml-property:TimeConstraint-specification .

mms-property:specificationInterval a mms-ontology:UmlObjectProperty ;
	mms-ontology:key "specificationId" ;
	rdfs:label "specificationInterval" ;
	rdfs:comment "The Interval that is the specification of this IntervalConstraint. Based on the UML property 'IntervalConstraint-specification' which is described as: The Interval that specifies the condition of the IntervalConstraint.."@en ;
	rdfs:domain uml-class:IntervalConstraint ;
	rdfs:range uml-class:Interval ;
	mms-ontology:umlPropertySource uml-property:IntervalConstraint-specification .

mms-property:specificationBehavioralFeature a mms-ontology:UmlObjectProperty ;
	mms-ontology:key "specificationId" ;
	rdfs:label "specificationBehavioralFeature" ;
	rdfs:comment "The BehavioralFeature that is the specification of this Behavior. Based on the UML property 'Behavior-specification' which is described as: Designates a BehavioralFeature that the Behavior implements. The BehavioralFeature must be owned by the BehavioredClassifier that owns the Behavior or be inherited by it. The Parameters of the BehavioralFeature and the implementing Behavior must match. A Behavior does not need to have a specification, in which case it either is the classifierBehavior of a BehavioredClassifier or it can only be invoked by another Behavior of the Classifier.."@en ;
	rdfs:domain uml-class:Behavior ;
	rdfs:range uml-class:BehavioralFeature ;
	mms-ontology:umlPropertySource uml-property:Behavior-specification .

mms-property:stateFromRegion a mms-ontology:UmlObjectProperty ;
	mms-ontology:key "stateId" ;
	rdfs:label "stateFromRegion" ;
	rdfs:comment "The State that belongs to this Region. Based on the UML property 'Region-state' which is described as: The State that owns the Region. If a Region is owned by a State, then it cannot also be owned by a StateMachine.."@en ;
	rdfs:domain uml-class:Region ;
	rdfs:range uml-class:State ;
	mms-ontology:umlPropertySource uml-property:Region-state .

mms-property:stateFromPseudostate a mms-ontology:UmlObjectProperty ;
	mms-ontology:key "stateId" ;
	rdfs:label "stateFromPseudostate" ;
	rdfs:comment "The State that belongs to this Pseudostate. Based on the UML property 'Pseudostate-state' which is described as: The State that owns this Pseudostate and in which it appears.."@en ;
	rdfs:domain uml-class:Pseudostate ;
	rdfs:range uml-class:State ;
	mms-ontology:umlPropertySource uml-property:Pseudostate-state .

mms-property:stateFromConnectionPointReference a mms-ontology:UmlObjectProperty ;
	mms-ontology:key "stateId" ;
	rdfs:label "stateFromConnectionPointReference" ;
	rdfs:comment "The State that belongs to this ConnectionPointReference. Based on the UML property 'ConnectionPointReference-state' which is described as: The State in which the ConnectionPointReference is defined.."@en ;
	rdfs:domain uml-class:ConnectionPointReference ;
	rdfs:range uml-class:State ;
	mms-ontology:umlPropertySource uml-property:ConnectionPointReference-state .

mms-property:stateInvariantConstraint a mms-ontology:UmlObjectProperty ;
	mms-ontology:key "stateInvariantId" ;
	rdfs:label "stateInvariantConstraint" ;
	rdfs:comment "The Constraint that is the stateInvariant of this State. Based on the UML property 'State-stateInvariant' which is described as: Specifies conditions that are always true when this State is the current State. In ProtocolStateMachines state invariants are additional conditions to the preconditions of the outgoing Transitions, and to the postcondition of the incoming Transitions.."@en ;
	rdfs:domain uml-class:State ;
	rdfs:range uml-class:Constraint ;
	mms-ontology:umlPropertySource uml-property:State-stateInvariant .

mms-property:stateMachineFromPseudostate a mms-ontology:UmlObjectProperty ;
	mms-ontology:key "stateMachineId" ;
	rdfs:label "stateMachineFromPseudostate" ;
	rdfs:comment "The StateMachine that belongs to this Pseudostate. Based on the UML property 'Pseudostate-stateMachine' which is described as: The StateMachine in which this Pseudostate is defined. This only applies to Pseudostates of the kind entryPoint or exitPoint.."@en ;
	rdfs:domain uml-class:Pseudostate ;
	rdfs:range uml-class:StateMachine ;
	mms-ontology:umlPropertySource uml-property:Pseudostate-stateMachine .

mms-property:stateMachineFromRegion a mms-ontology:UmlObjectProperty ;
	mms-ontology:key "stateMachineId" ;
	rdfs:label "stateMachineFromRegion" ;
	rdfs:comment "The StateMachine that belongs to this Region. Based on the UML property 'Region-stateMachine' which is described as: The StateMachine that owns the Region. If a Region is owned by a StateMachine, then it cannot also be owned by a State.."@en ;
	rdfs:domain uml-class:Region ;
	rdfs:range uml-class:StateMachine ;
	mms-ontology:umlPropertySource uml-property:Region-stateMachine .

mms-property:structuralFeature a mms-ontology:UmlObjectProperty ;
	mms-ontology:key "structuralFeatureId" ;
	rdfs:label "structuralFeature" ;
	rdfs:comment "The StructuralFeature that belongs to this StructuralFeatureAction. Based on the UML property 'StructuralFeatureAction-structuralFeature' which is described as: The StructuralFeature to be read or written.."@en ;
	rdfs:domain uml-class:StructuralFeatureAction ;
	rdfs:range uml-class:StructuralFeature ;
	mms-ontology:umlPropertySource uml-property:StructuralFeatureAction-structuralFeature .

mms-property:subpartition a mms-ontology:UmlObjectProperty ;
	mms-ontology:key "subpartitionIds" ;
	rdfs:label "subpartition" ;
	rdfs:comment "A ActivityPartition that is the subpartition of this ActivityPartition. Based on the UML property 'ActivityPartition-subpartition' which is described as: Other ActivityPartitions immediately contained in this ActivityPartition (as its subgroups).."@en ;
	rdfs:domain uml-class:ActivityPartition ;
	rdfs:range uml-class:ActivityPartition ;
	mms-ontology:umlPropertySource uml-property:ActivityPartition-subpartition .

mms-property:subsettedProperty a mms-ontology:UmlObjectProperty ;
	mms-ontology:key "subsettedPropertyIds" ;
	rdfs:label "subsettedProperty" ;
	rdfs:comment "A Property that belongs to this Property. Based on the UML property 'Property-subsettedProperty' which is described as: The properties of which this Property is constrained to be a subset, if any.."@en ;
	rdfs:domain uml-class:Property ;
	rdfs:range uml-class:Property ;
	mms-ontology:umlPropertySource uml-property:Property-subsettedProperty .

mms-property:subvertex a mms-ontology:UmlObjectProperty ;
	mms-ontology:key "subvertexIds" ;
	rdfs:label "subvertex" ;
	rdfs:comment "A Vertex that is the subvertex of this Region. Based on the UML property 'Region-subvertex' which is described as: The set of Vertices that are owned by this Region.."@en ;
	rdfs:domain uml-class:Region ;
	rdfs:range uml-class:Vertex ;
	mms-ontology:umlPropertySource uml-property:Region-subvertex .

mms-property:superPartitionActivityPartition a mms-ontology:UmlObjectProperty ;
	mms-ontology:key "superPartitionId" ;
	rdfs:label "superPartitionActivityPartition" ;
	rdfs:comment "The ActivityPartition that is the superPartition of this ActivityPartition. Based on the UML property 'ActivityPartition-superPartition' which is described as: Other ActivityPartitions immediately containing this ActivityPartition (as its superGroups).."@en ;
	rdfs:domain uml-class:ActivityPartition ;
	rdfs:range uml-class:ActivityPartition ;
	mms-ontology:umlPropertySource uml-property:ActivityPartition-superPartition .

mms-property:supplier a mms-ontology:UmlObjectProperty ;
	mms-ontology:key "supplierIds" ;
	rdfs:label "supplier" ;
	rdfs:comment "A NamedElement that is the supplier of this Dependency. Based on the UML property 'Dependency-supplier' which is described as: The Element(s) on which the client Element(s) depend in some respect. The modeler may stipulate a sense of Dependency direction suitable for their domain.."@en ;
	rdfs:domain uml-class:Dependency ;
	rdfs:range uml-class:NamedElement ;
	mms-ontology:umlPropertySource uml-property:Dependency-supplier .

mms-property:targetVertex a mms-ontology:UmlObjectProperty ;
	mms-ontology:key "targetId" ;
	rdfs:label "targetVertex" ;
	rdfs:comment "The Vertex that is the target of this Transition. Based on the UML property 'Transition-target' which is described as: Designates the target Vertex that is reached when the Transition is taken.."@en ;
	rdfs:domain uml-class:Transition ;
	rdfs:range uml-class:Vertex ;
	mms-ontology:umlPropertySource uml-property:Transition-target .

mms-property:targetInputPinFromSendSignalAction a mms-ontology:UmlObjectProperty ;
	mms-ontology:key "targetId" ;
	rdfs:label "targetInputPinFromSendSignalAction" ;
	rdfs:comment "The InputPin that is the target of this SendSignalAction. Based on the UML property 'SendSignalAction-target' which is described as: The InputPin that provides the target object to which the Signal instance is sent.."@en ;
	rdfs:domain uml-class:SendSignalAction ;
	rdfs:range uml-class:InputPin ;
	mms-ontology:umlPropertySource uml-property:SendSignalAction-target .

mms-property:targetInputPinFromCallOperationAction a mms-ontology:UmlObjectProperty ;
	mms-ontology:key "targetId" ;
	rdfs:label "targetInputPinFromCallOperationAction" ;
	rdfs:comment "The InputPin that is the target of this CallOperationAction. Based on the UML property 'CallOperationAction-target' which is described as: The InputPin that provides the target object to which the Operation call request is sent.."@en ;
	rdfs:domain uml-class:CallOperationAction ;
	rdfs:range uml-class:InputPin ;
	mms-ontology:umlPropertySource uml-property:CallOperationAction-target .

mms-property:targetInputPinFromSendObjectAction a mms-ontology:UmlObjectProperty ;
	mms-ontology:key "targetId" ;
	rdfs:label "targetInputPinFromSendObjectAction" ;
	rdfs:comment "The InputPin that is the target of this SendObjectAction. Based on the UML property 'SendObjectAction-target' which is described as: The target object to which the object is sent.."@en ;
	rdfs:domain uml-class:SendObjectAction ;
	rdfs:range uml-class:InputPin ;
	mms-ontology:umlPropertySource uml-property:SendObjectAction-target .

mms-property:targetInputPinFromDestroyObjectAction a mms-ontology:UmlObjectProperty ;
	mms-ontology:key "targetId" ;
	rdfs:label "targetInputPinFromDestroyObjectAction" ;
	rdfs:comment "The InputPin that is the target of this DestroyObjectAction. Based on the UML property 'DestroyObjectAction-target' which is described as: The InputPin providing the object to be destroyed.."@en ;
	rdfs:domain uml-class:DestroyObjectAction ;
	rdfs:range uml-class:InputPin ;
	mms-ontology:umlPropertySource uml-property:DestroyObjectAction-target .

mms-property:targetActivityNode a mms-ontology:UmlObjectProperty ;
	mms-ontology:key "targetId" ;
	rdfs:label "targetActivityNode" ;
	rdfs:comment "The ActivityNode that is the target of this ActivityEdge. Based on the UML property 'ActivityEdge-target' which is described as: The ActivityNode to which tokens are put when they traverse the ActivityEdge.."@en ;
	rdfs:domain uml-class:ActivityEdge ;
	rdfs:range uml-class:ActivityNode ;
	mms-ontology:umlPropertySource uml-property:ActivityEdge-target .

mms-property:targetElement a mms-ontology:UmlObjectProperty ;
	mms-ontology:key "targetId" ;
	rdfs:label "targetElement" ;
	rdfs:comment "The Element that is the target of this DirectedRelationship. Based on the UML property 'DirectedRelationship-target' which is described as: Specifies the target Element(s) of the DirectedRelationship.."@en ;
	rdfs:domain uml-class:DirectedRelationship ;
	rdfs:range uml-class:Element ;
	mms-ontology:umlPropertySource uml-property:DirectedRelationship-target .

mms-property:testFromLoopNode a mms-ontology:UmlObjectProperty ;
	mms-ontology:key "testIds" ;
	rdfs:label "testFromLoopNode" ;
	rdfs:comment "A ExecutableNode that is the test of this LoopNode. Based on the UML property 'LoopNode-test' which is described as: The set of ExecutableNodes executed in order to provide the test result for the loop.."@en ;
	rdfs:domain uml-class:LoopNode ;
	rdfs:range uml-class:ExecutableNode ;
	mms-ontology:umlPropertySource uml-property:LoopNode-test .

mms-property:testFromClause a mms-ontology:UmlObjectProperty ;
	mms-ontology:key "testIds" ;
	rdfs:label "testFromClause" ;
	rdfs:comment "A ExecutableNode that is the test of this Clause. Based on the UML property 'Clause-test' which is described as: The set of ExecutableNodes that are executed in order to provide a test result for the Clause.."@en ;
	rdfs:domain uml-class:Clause ;
	rdfs:range uml-class:ExecutableNode ;
	mms-ontology:umlPropertySource uml-property:Clause-test .

mms-property:transition a mms-ontology:UmlObjectProperty ;
	mms-ontology:key "transitionIds" ;
	rdfs:label "transition" ;
	rdfs:comment "A Transition that belongs to this Region. Based on the UML property 'Region-transition' which is described as: The set of Transitions owned by the Region.."@en ;
	rdfs:domain uml-class:Region ;
	rdfs:range uml-class:Transition ;
	mms-ontology:umlPropertySource uml-property:Region-transition .

mms-property:triggerFromTransition a mms-ontology:UmlObjectProperty ;
	mms-ontology:key "triggerIds" ;
	rdfs:label "triggerFromTransition" ;
	rdfs:comment "A Trigger that belongs to this Transition. Based on the UML property 'Transition-trigger' which is described as: Specifies the Triggers that may fire the transition.."@en ;
	rdfs:domain uml-class:Transition ;
	rdfs:range uml-class:Trigger ;
	mms-ontology:umlPropertySource uml-property:Transition-trigger .

mms-property:triggerFromAcceptEventAction a mms-ontology:UmlObjectProperty ;
	mms-ontology:key "triggerIds" ;
	rdfs:label "triggerFromAcceptEventAction" ;
	rdfs:comment "A Trigger that belongs to this AcceptEventAction. Based on the UML property 'AcceptEventAction-trigger' which is described as: The Triggers specifying the Events of which the AcceptEventAction waits for occurrences.."@en ;
	rdfs:domain uml-class:AcceptEventAction ;
	rdfs:range uml-class:Trigger ;
	mms-ontology:umlPropertySource uml-property:AcceptEventAction-trigger .

mms-property:typeFromTypedElement a mms-ontology:UmlObjectProperty ;
	mms-ontology:key "typeId" ;
	rdfs:label "typeFromTypedElement" ;
	rdfs:comment "The Type that belongs to this TypedElement. Based on the UML property 'TypedElement-type' which is described as: The type of the TypedElement.."@en ;
	rdfs:domain uml-class:TypedElement ;
	rdfs:range uml-class:Type ;
	mms-ontology:umlPropertySource uml-property:TypedElement-type .

mms-property:typeFromOperation a mms-ontology:UmlObjectProperty ;
	mms-ontology:key "typeId" ;
	rdfs:label "typeFromOperation" ;
	rdfs:comment "The Type that belongs to this Operation. Based on the UML property 'Operation-type' which is described as: The return type of the operation, if present. This information is derived from the return result for this Operation.."@en ;
	rdfs:domain uml-class:Operation ;
	rdfs:range uml-class:Type ;
	mms-ontology:umlPropertySource uml-property:Operation-type .

mms-property:typeStereotype a mms-ontology:UmlObjectProperty ;
	mms-ontology:key "typeId" ;
	rdfs:label "typeStereotype" ;
	rdfs:comment "The Stereotype that is the type of this ExtensionEnd. Based on the UML property 'ExtensionEnd-type' which is described as: References the type of the ExtensionEnd. Note that this association restricts the possible types of an ExtensionEnd to only be Stereotypes.."@en ;
	rdfs:domain uml-class:ExtensionEnd ;
	rdfs:range uml-class:Stereotype ;
	mms-ontology:umlPropertySource uml-property:ExtensionEnd-type .

mms-property:typeAssociation a mms-ontology:UmlObjectProperty ;
	mms-ontology:key "typeId" ;
	rdfs:label "typeAssociation" ;
	rdfs:comment "The Association that is the type of this Connector. Based on the UML property 'Connector-type' which is described as: An optional Association that classifies links corresponding to this Connector.."@en ;
	rdfs:domain uml-class:Connector ;
	rdfs:range uml-class:Association ;
	mms-ontology:umlPropertySource uml-property:Connector-type .

mms-property:typeCollaboration a mms-ontology:UmlObjectProperty ;
	mms-ontology:key "typeId" ;
	rdfs:label "typeCollaboration" ;
	rdfs:comment "The Collaboration that is the type of this CollaborationUse. Based on the UML property 'CollaborationUse-type' which is described as: The Collaboration which is used in this CollaborationUse. The Collaboration defines the cooperation between its roles which are mapped to ConnectableElements relating to the Classifier owning the CollaborationUse.."@en ;
	rdfs:domain uml-class:CollaborationUse ;
	rdfs:range uml-class:Collaboration ;
	mms-ontology:umlPropertySource uml-property:CollaborationUse-type .

mms-property:valueBoolean a mms-ontology:UmlObjectProperty ;
	mms-ontology:key "valueId" ;
	rdfs:label "valueBoolean" ;
	rdfs:comment "The Boolean that is the value of this LiteralBoolean. Based on the UML property 'LiteralBoolean-value' which is described as: The specified Boolean value.."@en ;
	rdfs:domain uml-class:LiteralBoolean ;
	rdfs:range uml-primitives:Boolean ;
	mms-ontology:umlPropertySource uml-property:LiteralBoolean-value .

mms-property:valueValueSpecificationFromValuePin a mms-ontology:UmlObjectProperty ;
	mms-ontology:key "valueId" ;
	rdfs:label "valueValueSpecificationFromValuePin" ;
	rdfs:comment "The ValueSpecification that is the value of this ValuePin. Based on the UML property 'ValuePin-value' which is described as: The ValueSpecification that is evaluated to obtain the value that the ValuePin will provide.."@en ;
	rdfs:domain uml-class:ValuePin ;
	rdfs:range uml-class:ValueSpecification ;
	mms-ontology:umlPropertySource uml-property:ValuePin-value .

mms-property:valueValueSpecificationFromValueSpecificationAction a mms-ontology:UmlObjectProperty ;
	mms-ontology:key "valueId" ;
	rdfs:label "valueValueSpecificationFromValueSpecificationAction" ;
	rdfs:comment "The ValueSpecification that is the value of this ValueSpecificationAction. Based on the UML property 'ValueSpecificationAction-value' which is described as: The ValueSpecification to be evaluated.."@en ;
	rdfs:domain uml-class:ValueSpecificationAction ;
	rdfs:range uml-class:ValueSpecification ;
	mms-ontology:umlPropertySource uml-property:ValueSpecificationAction-value .

mms-property:valueValueSpecificationFromSlot a mms-ontology:UmlObjectProperty ;
	mms-ontology:key "valueId" ;
	rdfs:label "valueValueSpecificationFromSlot" ;
	rdfs:comment "The ValueSpecification that is the value of this Slot. Based on the UML property 'Slot-value' which is described as: The value or values held by the Slot.."@en ;
	rdfs:domain uml-class:Slot ;
	rdfs:range uml-class:ValueSpecification ;
	mms-ontology:umlPropertySource uml-property:Slot-value .

mms-property:valueInteger a mms-ontology:UmlObjectProperty ;
	mms-ontology:key "valueId" ;
	rdfs:label "valueInteger" ;
	rdfs:comment "The Integer that is the value of this LiteralInteger. Based on the UML property 'LiteralInteger-value' which is described as: The specified Integer value.."@en ;
	rdfs:domain uml-class:LiteralInteger ;
	rdfs:range uml-primitives:Integer ;
	mms-ontology:umlPropertySource uml-property:LiteralInteger-value .

mms-property:valueInputPinFromLinkEndData a mms-ontology:UmlObjectProperty ;
	mms-ontology:key "valueId" ;
	rdfs:label "valueInputPinFromLinkEndData" ;
	rdfs:comment "The InputPin that is the value of this LinkEndData. Based on the UML property 'LinkEndData-value' which is described as: The InputPin that provides the specified value for the given end. This InputPin is omitted if the LinkEndData specifies the &#34;open&#34; end for a ReadLinkAction.."@en ;
	rdfs:domain uml-class:LinkEndData ;
	rdfs:range uml-class:InputPin ;
	mms-ontology:umlPropertySource uml-property:LinkEndData-value .

mms-property:valueInputPinFromQualifierValue a mms-ontology:UmlObjectProperty ;
	mms-ontology:key "valueId" ;
	rdfs:label "valueInputPinFromQualifierValue" ;
	rdfs:comment "The InputPin that is the value of this QualifierValue. Based on the UML property 'QualifierValue-value' which is described as: The InputPin from which the specified value for the qualifier is taken.."@en ;
	rdfs:domain uml-class:QualifierValue ;
	rdfs:range uml-class:InputPin ;
	mms-ontology:umlPropertySource uml-property:QualifierValue-value .

mms-property:valueInputPinFromWriteStructuralFeatureAction a mms-ontology:UmlObjectProperty ;
	mms-ontology:key "valueId" ;
	rdfs:label "valueInputPinFromWriteStructuralFeatureAction" ;
	rdfs:comment "The InputPin that is the value of this WriteStructuralFeatureAction. Based on the UML property 'WriteStructuralFeatureAction-value' which is described as: The InputPin that provides the value to be added or removed from the StructuralFeature.."@en ;
	rdfs:domain uml-class:WriteStructuralFeatureAction ;
	rdfs:range uml-class:InputPin ;
	mms-ontology:umlPropertySource uml-property:WriteStructuralFeatureAction-value .

mms-property:valueInputPinFromWriteVariableAction a mms-ontology:UmlObjectProperty ;
	mms-ontology:key "valueId" ;
	rdfs:label "valueInputPinFromWriteVariableAction" ;
	rdfs:comment "The InputPin that is the value of this WriteVariableAction. Based on the UML property 'WriteVariableAction-value' which is described as: The InputPin that gives the value to be added or removed from the Variable.."@en ;
	rdfs:domain uml-class:WriteVariableAction ;
	rdfs:range uml-class:InputPin ;
	mms-ontology:umlPropertySource uml-property:WriteVariableAction-value .

mms-property:valueString a mms-ontology:UmlObjectProperty ;
	mms-ontology:key "valueId" ;
	rdfs:label "valueString" ;
	rdfs:comment "The String that is the value of this LiteralString. Based on the UML property 'LiteralString-value' which is described as: The specified String value.."@en ;
	rdfs:domain uml-class:LiteralString ;
	rdfs:range uml-primitives:String ;
	mms-ontology:umlPropertySource uml-property:LiteralString-value .

mms-property:valueReal a mms-ontology:UmlObjectProperty ;
	mms-ontology:key "valueId" ;
	rdfs:label "valueReal" ;
	rdfs:comment "The Real that is the value of this LiteralReal. Based on the UML property 'LiteralReal-value' which is described as: The specified Real value.."@en ;
	rdfs:domain uml-class:LiteralReal ;
	rdfs:range uml-primitives:Real ;
	mms-ontology:umlPropertySource uml-property:LiteralReal-value .

mms-property:valueUnlimitedNatural a mms-ontology:UmlObjectProperty ;
	mms-ontology:key "valueId" ;
	rdfs:label "valueUnlimitedNatural" ;
	rdfs:comment "The UnlimitedNatural that is the value of this LiteralUnlimitedNatural. Based on the UML property 'LiteralUnlimitedNatural-value' which is described as: The specified UnlimitedNatural value.."@en ;
	rdfs:domain uml-class:LiteralUnlimitedNatural ;
	rdfs:range uml-primitives:UnlimitedNatural ;
	mms-ontology:umlPropertySource uml-property:LiteralUnlimitedNatural-value .

